separated file

src/ClConv.v
@@ -1,191 +1,154 @@
-Require Import List PeanoNat Program.Basics FunctionalExtensionality.
+Require String.
+Import String.StringSyntax.
+Require Import List FunctionalExtensionality Arith.
+Require Import StateMachines.Inhabit StateMachines.Foldable.
 Import ListNotations.
 Set Universe Polymorphism.
 Open Scope type_scope.
+Open Scope string_scope.
 Set Implicit Arguments.
 
-Class habitable (A : Type) :=
-  { inhabitat : A }.
+Arguments existT {_ _} _ _.
 
-Instance nat_habitable : habitable nat :=
-  { inhabitat := 0 }.
+Section Effect.
+  Context (eff : Set)(args rets: eff -> Set)(ret_type : Set).
 
-Instance list_habitable (A : Type) : habitable (list A) :=
-  { inhabitat := @nil A }.
+  Inductive t :=
+  | Eff : forall (e : eff), args e -> (rets e -> t) -> t
+  | Return : ret_type -> t.
 
-Instance pair_habitable (A B : Type) `(HA : habitable A, HB : habitable B) : habitable (A * B) :=
-  { inhabitat := (inhabitat,inhabitat) }.
+  Definition step_type (state : Set) := state -> forall (e : eff),
+      rets e -> (state * option { e : eff & args e }) + ret_type.
 
-Instance unit_habitable : habitable unit :=
-  { inhabitat := tt }.
+  Inductive equiv' (state : Set)(step : step_type state) :
+    state -> t -> option { e : eff & args e } -> Prop :=
+  | Equiv'Eff : forall s e (a : args e) p next op,
+      (forall r, equiv' step (next r) (p r) (op r)) ->
+      (forall r, step s e r = inl (next r, op r)) ->
+      equiv' step s (Eff a p) (Some (existT _ a))
+  | Equiv'Return : forall s o,
+      step s = (fun _ _ => inr o) ->
+      equiv' step s (Return o) None.
 
-Opaque inhabitat.
+  Definition equiv state (step : step_type state) init p :=
+    exists op s, step init = (fun _ _ => inl (s, op)) /\ equiv' step s p op.
 
-Definition sum_merge (A B C : Type)(f : A -> C)(g : B -> C)(x : sum A B) :=
+End Effect.
+
+Inductive effect := getNat | putNat | getString | putString | getRand.
+
+Scheme Equality for effect.
+
+Definition args_effect (e : effect) :=
+  match e with
+  | getNat => unit
+  | putNat => nat
+  | getString => unit
+  | putString => String.string
+  | getRand => unit
+  end.
+
+Definition rets_effect (e : effect) :=
+  match e with
+  | getNat => nat
+  | putNat => unit
+  | getString => String.string
+  | putString => unit
+  | getRand => list Ascii.ascii
+  end.
+
+Inductive yield_effect := yield : yield_effect.
+
+Notation "'const_yield' A" :=
+  (fun _:yield_effect => A)
+    (at level 10).
+
+Class is_eff eff :=
+  { args : eff -> Set;
+    rets : eff -> Set;
+    lift_eff : forall A B (e : eff)(_:rets e -> A + option B)(e0:eff),
+        rets e0 -> A + option B }.
+
+Definition equiv_coro A B state
+           (step : step_type (const_yield A)(const_yield B) unit state) init p :=
+  exists op s, forall r,
+      step init yield r = inl (s r, op r)
+      /\ equiv' (ret_type := unit) step (s r) (p r) (op r).
+
+Definition seqE (A B C:Set) (e : t (const_yield A) (const_yield B) unit)
+  : (A -> (B -> t (const_yield A) (const_yield B) unit) ->
+     t args_effect rets_effect (option C)) ->
+    t args_effect rets_effect (option C) :=
+  match e with
+  | Return _ _ c => fun _ => Return _ _ None
+  | Eff _ a p => fun cont => cont a p
+  end.
+
+Definition coro_type A B state
+           (_ : step_type (const_yield A) (const_yield B) unit state):=
+  B -> t (const_yield A)(const_yield B) unit.
+
+Definition proc_coro (A B C state : Set)
+           (step : step_type (const_yield A)(const_yield B) unit state)
+           (c : coro_type step) (x : B)
+  : (A -> coro_type step -> t args_effect rets_effect (option C)) ->
+    t args_effect rets_effect (option C) :=
+  seqE (c x).
+
+
+Fixpoint bind (T S eff : Set)(args rets : eff -> Set)
+         (x : t args rets T)(p : T -> t args rets S) :=
+  match x with
+  | Return _ _ v => p v
+  | Eff e a q => Eff e a (fun b => bind (q b) p)
+  end.
+
+Notation "n <- 'getN' ; e" :=
+  (Eff getNat (tt : args_effect getNat) (fun n : rets_effect getNat => e))
+    (at level 100, right associativity).
+Notation "'putN' n ; e" :=
+  (Eff putNat (n : args_effect putNat) (fun _ => e))
+    (at level 200).
+Notation "s <- 'getStr' ; e" :=
+  (Eff getString tt (fun s => e))
+    (at level 100, right associativity).
+Notation "'putStr' s ; e" :=
+  (Eff putString s (fun _ => e))
+    (at level 200).
+Notation "n <- 'resume' c $ x ; e" :=
+  (proc_coro c x (fun n c => e))
+    (at level 100, right associativity).
+Notation "v1 <- 'yield' v2 ; e" :=
+  (Eff yield v2 (fun v1 => e))
+    (at level 100, right associativity).
+Notation "x <- 'getRnd' ; e" :=
+  (Eff getRand (tt : args_effect getRand) (fun x : rets_effect getRand => e))
+    (at level 100, right associativity).
+Notation "x <<- p ; e" :=
+  (bind p (fun x => e))
+    (at level 100, right associativity).
+
+Definition get_put : t args_effect rets_effect nat :=
+  n <- getN;
+  putN (S n);
+  Return _ _ (S n).
+
+Definition seqE' A C state
+           (x : (state * option { e : yield_effect & A }) + unit)
+           (f : state -> A -> t args_effect rets_effect C)
+           (f0 : t args_effect rets_effect C) :=
+  match x with
+  | inl (s, Some (existT _ v)) => f s v
+  | _ => f0
+  end.
+
+Definition sum_merge (A B C : Set)(f : A -> C)(g : B -> C)(x : sum A B) :=
   match x with
   | inl a => f a
   | inr b => g b
   end.
 
-Definition LetIn (A B : Type) (f:A -> B) (x:A) := f x.
-Notation "'Let' x := def 'in' body" := (LetIn (fun x => body) def) (at level 100).
-
 Infix "|||" := sum_merge (at level 60).
-
-Inductive t (eff : Type -> Type) (a : Type) :=
-| Pure : a -> t eff a
-| Eff : forall T, eff T -> (T -> t eff a) -> t eff a.
-
-Inductive effect : Type -> Type :=
-| getE : unit -> effect nat
-| putE : nat -> effect unit
-| readE : unit -> effect (list nat)
-| printE : list nat -> effect unit
-| genKeyE : unit -> effect (list nat * list nat).
-
-Notation "n <- 'get' ; e" := (Eff (getE tt) (fun n => e)) (at level 200, right associativity).
-Notation "'put' n ; e" := (Eff (putE n) (fun _ => e)) (at level 200).
-Notation "'( k1 , k2 ) <- 'genKey' ; e" := (Eff (genKeyE tt) (fun k => let k1 := fst k in let k2 := snd k in e)) (at level 200, right associativity).
-Notation "l <- 'read' ; e" := (Eff (readE tt) (fun l => e)) (at level 200, right associativity).
-Notation "'print' l ; e" := (Eff (printE l) (fun _ => e)) (at level 200, right associativity).
-
-Inductive Coroutine (a b : Type):=
-  Co : (b -> t effect (CoroutineState a b)) -> Coroutine a b
-with CoroutineState (a b : Type) :=
-  Done : a -> CoroutineState a b
-| Suspend : a -> Coroutine a b -> CoroutineState a b.
-
-Definition suspend (a b : Type)(x : a)(c : Coroutine a b) :=
-  Pure effect (Suspend x c).
-
-Notation "'yield' x ; y <- 'input' ; e" :=
-  (suspend x (Co (fun y => e))) (at level 200, right associativity).
-Notation "'return' x" :=
-  (Pure _ (Done _ x)) (at level 200).
-
-Fixpoint seqE a b (e : t effect a)(f : a -> t effect b) : t effect b :=
-  match e with
-  | Pure _ x => f x
-  | Eff ef next =>
-    Eff ef (fun x => seqE (next x) f)
-  end.
-
-Notation "n <- 'resume' c $ x ; e" :=
-  (match c with
-  | Co e' =>
-   seqE (e' x) (fun s =>
-    match s with
-    | Done _ n => e
-    | Suspend n c => e
-    end)
-  end) (at level 100, right associativity).
-
-Definition coroutine_ex :=
-  Co (fun n =>
-        put n;
-        yield n;
-        m <- input;
-        put (n+m)%nat;
-        yield (n+m)%nat;
-        k <- input;
-        put (n+m+k)%nat;
-        return (n+m+k)%nat).
-
-Definition ex :=
-  let c := coroutine_ex in
-  n <- resume c $ 1;
-  put (10 * n)%nat;
-  k <- resume c $ 2;
-  put (10 * k)%nat;
-  s <- resume c $ 3;
-  put (10 * s)%nat;
-  Pure _ tt.
-
-Eval cbv in ex.
-(*
-     = put 1; (put 10; (put 3; (put 30; (put 6; (put 60; Pure effect tt)))))
-     : t effect unit
-*)
-
-Definition step_range (state : Type) :=
-  option {ty : Type & effect ty * (ty -> state) }.
-
-Inductive equiv (state a : Type)(step : state -> step_range state) :
-  state -> t effect a -> Prop :=
-| EquivEff :
-    forall (current : state)(T : Type)(next : T -> state)
-           (prog : T -> t effect a)(e : effect T),
-      step current = Some (existT _ _ (e, next)) ->
-      (forall x : T, equiv step (next x) (prog x)) ->
-      equiv step current (Eff e prog)
-| EquivPure :
-    forall (current : state)(x : a),
-      step current = None ->
-      equiv step current (Pure _ x).
-
-Ltac mem x__ env :=
-  lazymatch x__ with
-  | O => false
-  | tt => false
-  | _ =>
-    lazymatch env with
-    | context[x__] => true
-    | _ => false
-    end
-  end.
-
-Class reify_cls (A : Type)(x : A) := do_reify : A.
-
-Global Hint Extern 0 (@reify_cls _ _)
-=> (intros;
-      lazymatch goal with
-      | [ |- @reify_cls _ ?x ]
-        => exact x
-end) : typeclass_instances.
-
-Ltac merge t1 t2 :=
-  lazymatch t2 with
-  | (?t2',?x) =>
-    let t := merge t1 t2' in
-    let b := mem x t1 in
-    lazymatch b with
-    | true => constr:(t)
-    | false => constr:((t,x))
-    end
-  | tt => constr:(t1)
-  end.
-
-Definition Fix (A:Type)(t:A) := t.
-Definition label (A:Type)(_:A) := True.
-Definition label' (A:Type)(_:A) := True.
-
-Ltac put_label x :=
-  assert (label x) by (unfold label; auto).
-
-Ltac free_var exp env :=
-  let rec aux exp env :=
-      lazymatch env with
-      | (?env',?x) =>
-        lazymatch exp with
-        | context[x] =>
-          let env'' := aux exp env' in
-          constr:((env'',x))
-        | _ =>
-          aux exp env'
-        end
-      | _ => tt
-      end
-  in
-  let e := aux exp env in
-  e.
-
-Ltac remove a t :=
-  lazymatch t with
-  | (?t',a) => t'
-  | (?t',?x) =>
-    let v := remove a t' in
-    constr:((v,x))
-  end.
 
 Ltac curry_lhs :=
   lazymatch goal with
@@ -203,14 +166,13 @@ Ltac curry_lhs :=
   end.
 
 Ltac pattern_rhs term :=
-  match goal with
+  lazymatch goal with
     |- _ = ?X =>
-    let x := fresh in
-    set (x := X); pattern term in x; subst x
+    let X' := (eval pattern term in X) in
+    change X with X'
   end.
 
-
-Lemma equal_f : forall (A B : Type)(f g : A -> B) x,
+Lemma equal_f : forall (A B : Set)(f g : A -> B) x,
     f = g -> f x = g x.
   intros.
   congruence.
@@ -226,8 +188,7 @@ Ltac unify_fun :=
         | tt =>
           lazymatch goal with
           | |- _ = ?X =>
-            let tmp := fresh in
-            set (tmp := X); pattern tt at 0 in tmp; subst tmp
+            change X with ((fun _:unit => X) tt)
           end
          | _ =>
            tryif is_var x then
@@ -246,543 +207,1623 @@ Ltac unify_fun :=
   unify_fun_aux.
 
 Ltac dest_sum :=
-  match goal with
-  | |- ?g (@inl ?A ?B _) = ?t =>
-    let T := type of t in
-    let e := open_constr:((_|||_): A + B -> T) in
+  lazymatch goal with
+  | |- ?g (inl _) _ _ = ?t =>
+    let e := open_constr:(_|||_) in
+    unify g e
+  | |- ?g (inr _) _ _ = _ =>
+    let e := open_constr:(_|||_) in
+    unify g e
+  | |- ?g (inl _) = ?t =>
+    let e := open_constr:(_|||_) in
     unify g e
   | |- ?g (inr _) = _ =>
-    let ty := type of g in
-    let e := open_constr:((_|||_): ty) in
+    let e := open_constr:(_|||_) in
     unify g e
   end.
 
-Ltac dest_step :=
-  simpl;
-  repeat (dest_sum; simpl);
-  unify_fun.
-
-
-Ltac next_ptr state :=
-  lazymatch state with
-  | ?A + (?B + ?T) =>
-    let f := next_ptr T in
-    open_constr:(fun x => @inr A _ (@inr B _ (f x)))
-  | ?A + ?B => open_constr:(fun x => @inr A B x)
-  | ?A => open_constr:(fun x:A => x)
-  end.
-
-Ltac derive' env :=
-  lazymatch goal with
-  | |- @equiv ?state ?a ?step ?current ?p =>
-    lazymatch p with
-    | Pure _ _ =>
-      lazymatch current with
-      | apply _ _ => idtac
-      | ?f _ =>
-        let ptr := next_ptr state in
-        let e := open_constr:(fun _ => ptr (inl tt)) in
-        unify f e;
-        eapply EquivPure;
-        dest_step
-      end
-    | Eff ?e ?prog =>
-      lazymatch current with
-      | inl _ =>
-        eapply EquivEff;
-        [ dest_step | intros; derive' env ]
-      | ?f ?prev =>
-        let ptr := next_ptr state in
-        let ty := type of prev in
-        let fv := free_var p (env,prev) in
-        let H := fresh in
-        assert (label' fv) as H by (unfold label'; auto);
-        repeat match goal with
-               | X := ?def |- _ =>
-                 lazymatch def with
-                 | context [prev] =>
-                   progress (unfold X in H)
-                 end
-               end;
-        let fv_f :=
-            lazymatch goal with
-            | _: label' ?fv' |- _ =>
-              lazymatch (eval pattern prev in fv') with
-              | ?f _ => f
-              end
-            end
-        in
-        clear H;
-        let e := open_constr:(fun x:ty => ptr (inl (fv_f x))) in
-        let e' := (eval simpl in e) in
-        unify f e';
-        eapply EquivEff;
-        [ dest_step
-        | intros; derive' fv ]
-      end
-    | let (x1,x2) := ?x in _ =>
-      destruct x
-    | match ?m with O => _ | S m' => _ end =>
-      lazymatch current with
-      | ?f ?prev =>
-        let m' := fresh in
-        let ty := type of prev in
-        let e :=
-            lazymatch prev with
-            | m => open_constr:(fun x => match x return state with O => _ O | S m' => _ m' end)
-            | _ => open_constr:(match m return ty -> state with O => _ | S m' => _ end)
-            end
-        in
-        unify f e;
-        destruct m
-      end
-    | match ?m with None => _ | Some m' => _ end =>
-      lazymatch current with
-      | ?f ?prev =>
-        let m' := fresh in
-        let ty := type of prev in
-        lazymatch (eval pattern prev in m) with
-        | ?ctx _ =>
-          let e := open_constr:(fun x:ty => match ctx x return state with None => _ x | Some m' => _ x end) in
-          unify f e;
-          cbv beta;
-          destruct m
-        end
-      end
-    | (Let var := ?def in ?body) =>
-      lazymatch current with
-      | ?f ?prev =>
-        let v := fresh in
-        let ty := type of prev in
-        let e := open_constr:(fun x:ty => let v := def in _ x) in
-        unify f e;
-        set (v := def);
-        unfold LetIn
-      end
-    | ?fn ?m =>
-      lazymatch current with
-      | ?f ?prev =>
-        let rec aux fn accum :=
-            lazymatch fn with
-            | Fix ?fx =>
-              let ty := type of prev in
-              let x' := fresh "x" in
-              let H := fresh in
-              assert (label' m) as H by (unfold label'; auto);
-              repeat match goal with
-                     | X := ?def |- _ =>
-                            lazymatch def with
-                            | context [prev] =>
-                              progress (unfold X in H)
-                            end
-                     end;
-              let mred :=
-                  lazymatch goal with
-                  | _: label' ?m' |- _ => m'
-                  end
-              in
-              clear H;
-              let mf :=
-                  lazymatch (eval pattern prev in mred) with
-                  | ?g _ => g
-                  end
-              in
-              let a := fresh in
-              let e :=
-                  lazymatch type of m with
-                  | nat =>
-                    open_constr:(fun x:ty =>
-                                   match mf x return state with
-                                   | O => _ x
-                                   | S x' => _ x
-                                   end)
-                  | list nat =>
-                    open_constr:(fun x:ty =>
-                                   match mf x return state with
-                                   | [] => _ x
-                                   | a::x' => _ x
-                                   end)
-                  end
-              in
-              let e' := (eval simpl in e) in
-              unify f e';
-              simpl;
-              repeat match goal with
-                     | X := _ |- _ =>
-                            progress (fold X)
-                     end;
-              let tmp := fresh in
-              let tmp' := fresh in
-              set (tmp := fn);
-              set (tmp' := step);
-              lazymatch goal with
-                |- equiv _ ?c _ =>
-                cut (label c); [|unfold label; auto];
-                pattern m at 1;
-                lazymatch goal with
-                  |- (fun n:nat => label ?body -> _) _ =>
-                  lazymatch constr:(_ : forall n:nat, @reify_cls _ body) with
-                  | ?res =>
-                    simpl; intros;
-                    let tmp'' := fresh in
-                    set (tmp'' := res);
-                    fold (tmp'' m);
-                    let m' := fresh in
-                    generalize m at 1 2 as m';
-                    subst tmp;
-                    subst tmp';
-                    subst tmp'';
-                    intro m';
-                    accum;
-                    unfold Fix at 1;
-                    put_label fx;
-                    induction m';
-                    intros
-                  end
-                | |- (fun l:list nat => label ?body -> _) _ =>
-                  lazymatch constr:(_: forall l:list nat, @reify_cls _ body) with
-                  | ?res =>
-                    simpl; intros;
-                    let tmp'' := fresh in
-                    set (tmp'' := res);
-                    fold (tmp'' m);
-                    let m' := fresh in
-                    generalize m at 1 2 as m';
-                    subst tmp;
-                    subst tmp';
-                    subst tmp'';
-                    intro m';
-                    accum;
-                    unfold Fix at 1;
-                    put_label fx;
-                    induction m';
-                    intros
-                  end
-                end
-              end
-            | ?fn' ?a =>
-              aux fn' ltac:(generalize a; accum)
-            | _ =>
-              let a := fresh in
-              let e := open_constr:(fun a => _) in
-              unify f e;
-              simpl;
-              eauto
-            end
-        in
-        aux fn idtac
-      end
+Ltac free_var body vars :=
+  lazymatch vars with
+  | (?rest,?a) =>
+    let r := free_var body rest in
+    lazymatch body with
+    | context [a] =>
+      constr:((r,a))
+    | _ => r
     end
+  | ?a => tt
   end.
 
-Theorem ex_derive :
-  {state & {step & {init | @equiv state _ step init ex}}}.
+Definition nat_rect_nondep A f (f0 : nat -> A -> A) :=
+  fix F (n : nat) : A :=
+    match n with
+    | O => f
+    | S n' => f0 n' (F n')
+    end.
+
+Definition list_rec_nondep A B fnil fcons :=
+  fix aux (l:list A) : B :=
+    match l with
+    | [] => fnil
+    | x::xs => fcons x xs (aux xs)
+    end.
+
+
+Definition ex_coroutine k n : t (const_yield nat) (const_yield nat) unit :=
+  m <- yield (k + n)%nat;
+    _ <- yield (n + m)%nat;
+    Return _ _ tt .
+
+Ltac st_op_to_ev :=
+  lazymatch goal with
+    |- equiv' ?step ?st ?prog ?op =>
+    lazymatch st with
+    | ?f _ _ =>
+      let u := open_constr:(fun r c => _) in
+      unify f u;
+      lazymatch op with
+      | ?g _ _ =>
+        let u := open_constr:(fun r c => _) in
+        unify g u
+      end
+    | ?f _ =>
+      let u := open_constr:(fun r => _) in
+      unify f u;
+      lazymatch op with
+      | ?g _ =>
+        let u := open_constr:(fun r => _) in
+        unify g u
+      end
+    | _ => idtac
+    end;
+    cbv beta
+  end.
+
+Lemma derive_parent_rect : forall state A C N (a0:A) f f0 st0 stS op0 opS step,
+    (forall a, equiv' step (st0 a) (f a a) (op0 a)) ->
+    (forall N0,
+        (forall a, equiv' step (match N0 with O => st0 a | S N0' => stS a N0' end) (nat_rect_nondep (f a) (f0 a) N0 a) (match N0 with O => op0 a | S N0' => opS a N0' end)) ->
+        (forall a, equiv' step (stS a N0)
+                          (f0 a N0
+                              (nat_rect_nondep
+                                    (f a) (f0 a)
+                                    N0) a) (opS a N0))) ->
+    @equiv' _ args_effect rets_effect C state step (match N with O => st0 a0 | S N0 => stS a0 N0 end) (nat_rect_nondep (f a0) (f0 a0) N a0) (match N with O => op0 a0 | S N0 => opS a0 N0 end).
 Proof.
-  do 2 eexists.
-  eexists ?[init].
-  unfold ex, coroutine_ex, seqE.
+  intros.
+  revert a0.
+  induction N; intros; simpl; auto.
+Qed.
+
+Lemma derive_list_rec : forall state A B C (l : list B)(a0:A) f f0 st0 stS op0 opS step,
+    (forall a, equiv' step (st0 a) (f a a) (op0 a)) ->
+    (forall b0 l0,
+        (forall a,
+            equiv' step
+                   (match l0 with [] => st0 a | b::l' => stS a b l' end)
+                   (list_rec_nondep (f a) (f0 a) l0 a)
+                   (match l0 with [] => op0 a | b::l' => opS a b l' end)) ->
+        (forall a, equiv' step (stS a b0 l0)
+                          (f0 a b0 l0
+                              (list_rec_nondep
+                                 (f a) (f0 a)
+                                 l0) a) (opS a b0 l0))) ->
+    @equiv' _ args_effect rets_effect C state step
+            (match l with [] => st0 a0 | b::l' => stS a0 b l' end)
+            (list_rec_nondep (f a0) (f0 a0) l a0)
+            (match l with [] => op0 a0 | b::l' => opS a0 b l' end).
+Proof.
+  intros.
+  revert a0.
+  induction l; intros; simpl; auto.
+Qed.
+
+Lemma derive_opt : forall eff args rets A C state (x : option A) sta st fa f opa op step,
+    (forall a, equiv' step (sta a) (fa a) (opa a)) ->
+    equiv' step st f op ->
+    @equiv' eff args rets C state step
+           (match x with Some a => sta a | None => st end)
+           (match x with Some a => fa a | None => f end)
+           (match x with Some a => opa a | None => op end).
+Proof.
+  intros.
+  destruct x; auto.
+Qed.
+
+Lemma derive_bool : forall eff args rets C state (b:bool) stt stf ft ff opt opf step,
+    equiv' step stt ft opt ->
+    equiv' step stf ff opf ->
+    @equiv' eff args rets C state step (if b then stt else stf)
+            (if b then ft else ff) (if b then opt else opf).
+Proof.
+  intros.
+  destruct b; auto.
+Qed.
+
+Lemma derive_sum : forall eff args rets A B C state (x : A + B) fa fb sta stb opa opb step,
+    (forall a, equiv' step (sta a) (fa a) (opa a)) ->
+    (forall b, equiv' step (stb b) (fb b) (opb b)) ->
+    @equiv' eff args rets C state step (match x with
+                                        | inl a => sta a
+                                        | inr b => stb b
+                                        end)
+            (match x with
+             | inl a => fa a
+             | inr b => fb b
+             end)
+            (match x with
+             | inl a => opa a
+             | inr b => opb b
+             end).
+Proof.
+  intros.
+  destruct x; auto.
+Qed.
+
+Lemma derive_seqE' :
+  forall A C state state'
+         (x : (state' * option { _ : yield_effect & A }) + unit)
+         f f0 g g0 h h0 step,
+    (forall s v, equiv' step (g s v) (f s v) (h s v)) ->
+    equiv' step g0 f0 h0 ->
+    @equiv' _ _ _ C state step
+            (match x with
+             | inl (s, Some (existT _ v)) => g s v
+             | _ => g0
+             end) (seqE' x f f0)
+            (match x with
+             | inl (s, Some (existT _ v)) => h s v
+             | _ => h0
+             end).
+Proof.
+  intros.
+  destruct x.
+  destruct p.
+  destruct o.
+  destruct s0.
   simpl.
-  let e := open_constr:(inl tt) in
-  unify ?init e.
-  unshelve derive' tt.
-  all: exact unit || exact (fun _ => None).
-Defined.
+  auto.
+  simpl.
+  auto.
+  simpl.
+  auto.
+Qed.
 
-Definition exLetIn : t effect unit :=
-  n <- get;
-    Let m := S n in put m; put m; Pure _ tt.
+Definition step_state (A B C state : Set)
+           (step : step_type (const_yield A)(const_yield B) unit state) st x g :=
+  seqE' (step st yield x) (fun s v => g v s) (Return _ _ (@None C)).
 
-Theorem exLetIn_derive :
-  {state & {step & {init | @equiv state _ step init exLetIn}}}.
+Lemma equal_f_dep : forall A (T : A -> Set) B (f g : forall a, T a -> B) a0,
+    f = g -> f a0 = g a0.
 Proof.
-  do 2 eexists.
-  eexists ?[init].
-  unfold exLetIn.
-  let e := open_constr:(inl tt) in
-  unify ?init e.
-  derive' tt.
-  unshelve derive' (tt,H).
-  all: exact unit || exact (fun _ => None).
-Defined.
-
-Eval cbv [exLetIn_derive exLetIn prod_curry sum_merge] in exLetIn_derive.
-
-Definition ex1 : t effect unit:=
-  n <- get;
-    put n;
-    put n;
-    Pure _ tt.
-
-Theorem ex1_derive : {state & {step & {init | @equiv state _ step init ex1}}}.
-Proof.
-  do 2 eexists.
-  eexists ?[init].
-  unfold ex1.
-  let e := open_constr:(inl tt) in
-  unify ?init e.
-  derive' tt.
-  Grab Existential Variables.
-  all: exact unit || exact (fun _ => None).
-Defined.
-
-Eval cbv [ex1_derive ex1 sum_merge projT2 projT1] in projT1 (projT2 ex1_derive).
-
-
-Goal {state & {step & {init | @equiv state _ step init
-                                     (n <- get;
-                                        m <- get;
-                                        match n with
-                                        | O => put 0; Pure _ tt
-                                        | S n' => put n'; Pure _ tt
-                                        end)}}}.
-Proof.
-  do 2 eexists.
-  eexists ?[init].
-  let e := open_constr:(inl tt) in
-  unify ?init e.
-  derive' tt.
-  derive' tt.
-  derive' (tt,x).
-  Grab Existential Variables.
-  all: exact unit || exact (fun _ => None).
-Defined.
-
-
-Definition readL (f : list nat -> t effect unit) :=
-  Fix (fix readL accum n :=
-         match n with
-         | O => f accum
-         | S n' =>
-           x <- get;
-             readL (accum ++ [x]) n'
-         end).
-
-
-Definition printL (e : t effect unit) :=
-  Fix (fix printL l :=
-    match l with
-    | [] => e
-    | a::l' =>
-      put a;
-        printL l'
-    end).
-
-Theorem ex3: {state & {step & {init | @equiv state _ step init
-                                             (m <- get;
-                                                n <- get;
-                                        Fix (fix f y :=
-                                           match y with
-                                           | O => put n; put m; Pure _ tt
-                                           | S y' => put y; f y'
-                                           end) (m+n)%nat)}}}.
-Proof.
-  do 2 eexists.
-  eexists ?[init].
-  let e := open_constr:(inl tt) in
-  unify ?init e.  
-  derive' tt.
-  derive' (tt,x,x0).
-  derive' (tt,H4,x,x0).
-  Grab Existential Variables.
-  all: exact unit || exact (fun _ => None).
-Defined.
-
-Theorem ex_read: {state & {step & forall l', {init |
-                       @equiv state _ step init
-                              (n <- get;
-                                 readL (fun l => put (length l); Pure _ tt)
-                                       l' n) }}}.
-Proof.
-  unfold readL.
-  do 2 eexists.
   intros.
-  eexists ?[init].
-  let e := open_constr:(inl (tt,l')) in
-  unify ?init e.
-  derive' (tt,l').
-  derive' (tt,l'0).
-  derive' (tt,l'0,H4).
-  Grab Existential Variables.
-  all: exact unit || exact (fun _ => None).
-Defined.
+  rewrite H.
+  auto.
+Qed.
 
-Eval cbv [prod_curry ex_read sum_merge projT1 projT2] in projT1 (projT2 ex_read).
+Ltac next_ptr :=
+  lazymatch goal with
+    |- @equiv' _ _ _ _ ?st _ _ _ _ =>
+    let rec aux state :=
+        lazymatch state with
+        | ?A + (?B + ?T) =>
+          let f := aux T in
+          open_constr:(fun x => @inr A _ (@inr B _ (f x)))
+        | ?A + ?B => open_constr:(fun x => @inr A B x)
+        | ?A => open_constr:(fun x:A => x)
+        end
+    in
+    aux st
+  end.
 
-Goal {state & {step & forall l,
-                  {init |
-                   @equiv state _ step init
-                          (put (length l); printL (Pure _ tt) l)}}}.
+Definition lift_effect A B(e : effect)(a : rets_effect e -> A + option B)(e0 : effect)
+  : rets_effect e0 -> A + option B :=
+  match
+  e as e1
+  return ((rets_effect e1 -> A + option B) -> rets_effect e0 -> A + option B)
+  with
+  | getNat =>
+    fun a0 : rets_effect getNat -> A + option B =>
+      match e0 as e1 return (rets_effect e1 -> A + option B) with
+      | getNat => a0
+      | _ => fun _ => inr None
+      end
+  | putNat =>
+    fun a0 : rets_effect putNat -> A + option B =>
+      match e0 as e1 return (rets_effect e1 -> A + option B) with
+      | putNat => a0
+      | _ => fun _ => inr None
+      end
+  | getString =>
+    fun a0 : rets_effect getString -> A + option B =>
+      match e0 as e1 return (rets_effect e1 -> A + option B) with
+      | getString => a0
+      | _ => fun _ => inr None
+      end
+  | putString =>
+    fun a0 : rets_effect putString -> A + option B =>
+      match e0 as e1 return (rets_effect e1 -> A + option B) with
+      | putString => a0
+      | _ => fun _ => inr None
+      end
+  | getRand =>
+    fun a0 : rets_effect getRand -> A + option B =>
+      match e0 as e1 return (rets_effect e1 -> A + option B) with
+      | getRand => a0
+      | _ => fun _ => inr None
+      end
+  end a.
+
+Instance effect_is_eff : is_eff effect :=
+  { args := args_effect;
+    rets := rets_effect;
+    lift_eff := lift_effect }.
+
+Ltac dest_step' :=
+  lazymatch goal with
+    |- @eq (?T1 + ?T2) (?g _ ?ef ?r) _ =>
+    pattern_rhs r;
+      apply equal_f;
+      lazymatch goal with
+        |- _ = ?rhs =>
+        lazymatch ef with
+          (*
+        | putNat =>
+          change rhs with
+          ((fun e => match e as e0 return rets_effect e0 -> T1+T2 with
+                     | putNat => rhs
+                     | _ => fun _ => inr None
+                     end) ef)
+        | getNat =>
+          change rhs with
+          ((fun e => match e as e0 return rets_effect e0 -> T1+T2 with
+                     | getNat => rhs
+                     | _ => fun _ => inr None
+                     end) ef)
+        | putString =>
+          change rhs with
+          ((fun e => match e as e0 return rets_effect e0 -> T1+T2 with
+                                | putString => rhs
+                                | _ => fun _ => inr None
+                                end) ef)
+        | getString =>
+          change rhs with
+          ((fun e => match e as e0 return rets_effect e0 -> T1+T2 with
+                                | getString => rhs
+                                | _ => fun _ => inr None
+                                end) ef)
+*)
+        | yield =>
+          (*
+          let tmp := fresh in
+          set (tmp := (fun _ => rhs yield));
+          replace rhs with tmp by (unfold tmp; auto);
+          subst tmp*)
+          change rhs with ((fun _ => rhs) yield)
+        | _ => change rhs with (lift_eff ef rhs ef)
+        end
+      end;
+      (apply equal_f_dep || apply equal_f);
+      simpl;
+      repeat (dest_sum; simpl);
+      unify_fun
+  | |- _ ?r = _ => repeat (dest_sum; simpl); unify_fun
+  end.
+
+Definition label := fun _:nat => True.
+
+Lemma bind_if : forall C D (b:bool)(p q : t args_effect rets_effect C)(r : C -> t args_effect rets_effect D),
+  bind (if b then p else q) r
+  = if b then bind p r else bind q r.
 Proof.
-  unfold printL.
-  do 2 eexists.
   intros.
-  eexists ?[init].
-  let e := open_constr:(inl (tt,l)) in
-  unify ?init e.
-  derive' (tt,l).
-  derive' tt.
-  derive' (tt, a, H4).
-  eapply IHlist.
-  Grab Existential Variables.
-  all: exact unit || exact (fun _ => None).
-Defined.
+  destruct b; auto.
+Qed.
 
-Goal {state & {step & forall l',
-                  {init |
-                   @equiv state _ step init
-                   (n <- get;
-                      readL (fun l => printL (Pure _ tt) l) l' n) }}}.
-Proof.
-  unfold readL, printL.
-  do 2 eexists.
-  intros.
-  eexists ?[init].
-  let e := open_constr:(inl (tt,l')) in
-  unify ?init e.
-  derive' (tt,l').
-  derive' (tt,l'0).
-  derive' tt.
-  derive' (tt,a,H6).
-  apply IHlist.
-  derive' (tt,l'0,H4).
-  Grab Existential Variables.
-  all: exact unit || exact (fun _ => None).
-Defined.
-
-Theorem ex4:
-  {state & {step & {init |
-                    @equiv state _ step init
-                           (k <- get;
-                              l <- get;
-                              n <- get;
-                              Fix (fix f z y x :=
-                                     match x with
-                                     | O =>
-                                       put y; Pure _ tt
-                                     | S x' =>
-                                       put 0;
-                                       f (S z) (z + y)%nat x'
-                                     end) l k n) }}}.
-Proof.
-  do 2 eexists.
-  eexists ?[init].
-  let e := open_constr:(inl tt) in
-  unify ?init e.
-  derive' tt.
-  derive' (tt,x2).
-  derive' (tt,x2,x3,H4).
-  Grab Existential Variables.
-  all: exact unit || exact (fun _ => None).
-Defined.
-
-Eval cbv [ex4 sum_merge prod_curry projT2 projT1] in projT1 (projT2 ex4).
-
-
-
-Parameter open : list nat -> list nat -> list nat -> list nat -> option (list nat).
-Parameter seal : list nat -> list nat -> list nat -> list nat -> list nat.
-
-Fixpoint splitAt A n (l : list A) :=
-  match n with
-  | O => ([], l)
-  | S n' =>
-    match l with
-    | [] => ([], [])
-    | x::l' =>
-      let (l1,l2) := splitAt n' l' in
-      (x::l1, l2)
+Ltac derive_core ptr env :=
+  st_op_to_ev;
+  lazymatch goal with
+    |- equiv' _ _ ?prog _ =>
+    let fv := free_var prog env in
+    lazymatch prog with
+    | @Eff _ ?args ?rets ?C ?e _ _ =>
+      eapply (Equiv'Eff (ptr (inl fv)) e);
+      [ let H := fresh in
+        intro H;
+        derive_core (fun x => ptr (inr x)) (env,H)
+       | intros; dest_step']
+    | Return _ _ _ =>
+      idtac
+      (*
+      eapply (Equiv'Return _ (ptr (inl fv)));
+      intros; cbv beta; dest_step'
+       *)
+    | bind (if _ then _ else _) _ =>
+      rewrite bind_if;
+      simpl;
+      derive_core ptr env
+    | seqE' _ _ _ =>
+      eapply (derive_seqE' _ (fun s v => _) (fun s v => _) (fun s v => _));
+      [ let s := fresh in
+        let v := fresh in
+        intros s v;
+        derive_core ptr (env,s,v)
+      | let ptr := next_ptr in
+        derive_core ptr env ]
+    | (match ?x with inl _ => _ end) =>
+      eapply (derive_sum _ _ _ (fun a => _) (fun b => _) (fun a => _) (fun b => _));
+      [ let a := fresh in
+        intro a;
+        cbv beta;
+        let ptr := next_ptr in
+        derive_core ptr (env,a)
+      | let b := fresh in
+        intro b;
+        cbv beta;
+        let ptr := next_ptr in
+        derive_core ptr (env,b)
+      ]
+    | (match ?x with Some _ => _ | None => _ end) =>
+      eapply (derive_opt _ (fun a => _) (fun a => _) (fun a => _));
+      [ let a := fresh in
+        intro a;
+        cbv beta;
+        let ptr := next_ptr in
+        derive_core ptr (env,a)
+      | cbv beta;
+        let ptr := next_ptr in
+        derive_core ptr env
+      ]
+    | (if ?b then _ else _) =>
+      eapply derive_bool;
+      [ let ptr := next_ptr in
+        derive_core ptr env
+      | let ptr := next_ptr in
+        derive_core ptr env
+      ]
+    | nat_rect_nondep _ _ _ _ =>
+      (now (repeat match goal with
+         | H : ?p |- _ => apply H
+         end))
+      ||
+      (eapply (derive_parent_rect _ _ (fun a b => _) (fun a => _) (fun a => _));
+       [ let a := fresh in
+         intro a;
+         cbv beta;
+         let ptr := next_ptr in
+         derive_core ptr (env,a)
+       | let n := fresh in
+         let H := fresh in
+         let a := fresh in
+         intros n H a;
+         cbv beta;
+         let ptr := next_ptr in
+         derive_core ptr (env,n,a)
+      ])
+    | list_rec_nondep _ _ _ _ =>
+      (now (repeat match goal with
+                   | H : ?p |- _ => apply H
+                   end))
+      ||
+      (eapply (derive_list_rec _ _ (fun _ _ => _) (fun _ => _) (fun _ => _));
+       [ let a := fresh in
+         intro a;
+         cbv beta;
+         let ptr := next_ptr in
+         derive_core ptr (env,a)
+       | let b := fresh in
+         let l := fresh in
+         let H := fresh in
+         let a := fresh in
+         intros b l H a;
+         cbv beta;
+         let ptr := next_ptr in
+         derive_core ptr (env,b,l,a)
+       ])
     end
   end.
 
 (*
-Notation "l <- 'read' ( l0 , n ) ; e" := (readL (fun l => e) l0 n) (at level 100, right associativity).
-Notation "'print' l ; e" := (printL e l) (at level 100, right associativity).
+Definition replace A i l (a:A) :=
+  (fix aux i l pre :=
+    match l with
+    | [] => []
+    | x::l' =>
+      match i with
+      | O => pre ++ a :: l'
+      | S i' => aux i' l' (pre ++ [x])
+      end
+    end) i l [].*)
+
+Definition pipe A B (a : A)(f : A -> B) := f a.
+
+Instance coro_type_inhabitant A B state step :
+  Inhabit (@coro_type A B state step) :=
+  { inhabitant := fun _ => Return _ _ inhabitant }.
+
+Instance t_inhabitant e a r (c:Set) `{IC : Inhabit c} : Inhabit (@t e a r c) :=
+  { inhabitant := Return _ _ inhabitant }.
+
+Definition seq_abs A B R state
+           (step : step_type (const_yield A)(const_yield B) R state) (x:B) C (_:C) (g : A -> C -> t args_effect rets_effect R ) := t_inhabitant.
+
+
+Opaque dummy.
+
+Definition equiv_coro' (A B C :Set) `{IA : Inhabit A} `{IB : Inhabit B} state
+           (step : step_type _ _ C state)
+           st
+           (coro : B -> t (const_yield A) (const_yield B) C) :=
+  exists op, equiv' step st (r <- yield inhabitant; coro r) op.
+
+Ltac get_init c :=
+  let init := open_constr:(_) in
+  let _ := constr:(ltac:(auto with equivc) : equiv_coro' _ init c) in
+  init.
+
+Ltac opt_match_fun expr :=
+  lazymatch expr with
+  | (match ?o with Some a => _ | None => _ end) =>
+    lazymatch (eval pattern o in expr) with
+    | ?F _ =>
+      eval cbv beta iota in (fun a => F (Some a))
+    end
+  end.
+
+Definition option_branch A B (f:A -> B) f0 o :=
+  match o with
+  | Some a => f a
+  | None => f0
+  end.
+
+Ltac to_dummy i p :=
+  lazymatch p with
+  | pipe ?c ?f =>
+    let init := get_init c in
+    let x := (eval cbv beta in (f (dummy _ _ i))) in
+    let d := to_dummy (S i) x in
+    lazymatch d with
+    | context [dummy _ ?T i] =>
+      lazymatch (eval pattern (dummy _ T i) in d) with
+      | ?g _ =>
+        constr:((pipe, init, g))
+      end
+    end
+  | @Eff _ args_effect rets_effect ?C ?e ?a ?f =>
+    let x := (eval cbv beta in (f (dummy _ _ i))) in
+    let d := to_dummy (S i) x in
+    lazymatch (eval pattern (dummy _ (rets_effect e) i) in d) with
+    | ?g _ =>
+      constr:((@Eff _ args_effect rets_effect C e a, g))
+    end
+  | @proc_coro ?A ?B ?C ?state ?step ?c ?z ?f =>
+    let x := (eval cbv beta in (f (dummy _ _ i) (dummy _ _ (S i)))) in
+    lazymatch f with
+    | context [proc_coro] =>
+      let d := to_dummy (S (S i)) x in
+      lazymatch type of f with
+      | _ -> ?T -> _ =>
+        lazymatch (eval pattern (dummy _ A i), (dummy _ T (S i)) in d) with
+        | ?g _ _ =>
+          constr:((@seq_abs A B C state step z (coro_type step) c, g))
+        end
+      end
+    | _ =>
+      constr:((@seq_abs A B C state step z (coro_type step) c, f))
+    end
+  | (match ?o with Some _ => _ | None => ?f0 end) =>
+    let f := opt_match_fun p in
+    lazymatch type of o with
+    | option ?A =>
+      let B := type of p in
+      let x := (eval cbv beta in (f (dummy _ _ i))) in
+      let d := to_dummy (S i) x in
+      let d0 := to_dummy i f0 in
+      lazymatch (eval pattern (dummy _ A i) in d) with
+      | ?g _ =>
+        constr:((@option_branch A B, g, d0, o))
+      end
+    end
+  | @nat_rect_nondep ?A ?f ?f0 ?n ?a =>
+    let x := (eval cbv beta in (f0 (dummy _ _ i) (dummy _ _ (S i)) (dummy _ _ (S (S i))))) in
+    let y := (eval cbv beta in (f (dummy _ _ i))) in
+    let d := to_dummy (S i) y in
+    let d0 := to_dummy (S (S (S i))) x in
+    let T := type of a in
+    lazymatch (eval pattern (dummy _ nat i), (dummy _ A (S i)), (dummy _ T (S (S i))) in d0) with
+    | ?g0 _ _ _ =>
+      lazymatch (eval pattern (dummy _ T i) in d) with
+      | ?g _ =>
+        constr:((@nat_rect_nondep A, g, g0, n, a))
+      end
+    end
+  | _ => p
+  end.
+
+Ltac reconstruct tree i :=
+  lazymatch tree with
+  | (pipe, ?init, ?f) =>
+    let x := (eval cbv beta in (f init)) in
+    reconstruct x i
+  | (Eff ?e ?a, ?p) =>
+    let x := (eval cbv beta in (p (dummy _ _ i))) in
+    let p' := reconstruct x (S i) in
+    lazymatch type of p with
+    | ?ty -> _ =>
+      lazymatch (eval pattern (dummy _ ty i) in p') with
+      | ?p'' _ =>
+        constr:(Eff e a p'')
+      end
+    end
+  | (@seq_abs ?A ?B ?C _ ?step ?z ?state ?st, ?p) =>
+    let x := (eval cbv beta in (p (dummy _ _ i) (dummy _ _ (S i)))) in
+    let p' := reconstruct x (S (S i)) in
+    lazymatch (eval pattern (dummy _ A i), (dummy _ state (S i)) in p') with
+    | ?p'' _ _ =>
+      constr:(@step_state A B C _ step st z p'')
+    end
+  | (@option_branch ?A ?B, ?f, ?f0, ?o) =>
+    let x := (eval cbv beta in (f (dummy _ _ i))) in
+    let p' := reconstruct x (S i) in
+    lazymatch (eval pattern (dummy _ A i) in p') with
+    | ?p'' _ =>
+      constr:(@option_branch A B p'' f0 o)
+    end
+  | (@nat_rect_nondep ?A, ?f, ?f0, ?n, ?a) =>
+    let x := (eval cbv beta in (f (dummy _ _ i))) in
+    let y := (eval cbv beta in (f0 (dummy _ _ i) (dummy _ _ (S i)) (dummy _ _ (S (S i))))) in
+    let f' := reconstruct x (S i) in
+    let f0' := reconstruct y (S (S (S i))) in
+    let ty := type of a in
+    lazymatch (eval pattern (dummy _ ty i) in f') with
+    | ?f'' _ =>
+      lazymatch (eval pattern (dummy _ nat i), (dummy _ A (S i)), (dummy _ ty (S (S i))) in f0') with
+      | ?f0'' _ _ _ =>
+        constr:(@nat_rect_nondep A f'' f0'' n a)
+      end
+    end
+  | _ => tree
+  end.
+
+Ltac coro_to_state p :=
+  let x := to_dummy 0 p in
+  lazymatch x with
+  | context [@coro_type _ _ ?state ?step] =>
+    lazymatch (eval pattern (coro_type step) in x) with
+    | ?F _ =>
+      let y := (eval cbv beta in (F state)) in
+      reconstruct y 0
+    end
+  end.
+
+Transparent proc_coro.
+
+(*
+Definition loop_ex (n i : nat)(g : forall A, A -> t args_effect rets_effect) :=
+  pipe (ex_coroutine 0 : coro_type (projT1 (projT2 ex_coroutine_derive')))
+       (fun c0 =>
+          nat_rect_nondep
+            (fun l =>
+               option_branch
+                        (fun c => g _ c)
+                        (Done _ _)
+                        (nth_err _ l i))
+            (fun m rec l =>
+               pipe (ex_coroutine m : coro_type (projT1 (projT2 ex_coroutine_derive')))
+                    (fun cm =>
+                       rec (cm::l)))
+            n [c0]).
 *)
-Definition foo :=
-  '(k1,k2) <- genKey;
-    put 0;
-    print k1;
-    print k2;
-    Pure _ tt.
+Ltac get_step c :=
+  let step := open_constr:(_) in
+  let _ := constr:(ltac:(auto with equivc') : equiv_coro' step _ c) in
+  step.
 
-Goal {state & {step & {init | @equiv state _ step init foo}}}.
-Proof.
-  unfold foo, printL.
-  do 2 eexists.
-  eexists ?[init].
-  let e := open_constr:(inl tt) in
-  unify ?init e.
-  derive' tt.
-  Grab Existential Variables.
-  all: exact unit || exact (fun _ => None).
+Ltac derive_coro env :=
+  lazymatch goal with
+    |- equiv _ _ ?x =>
+    let y := eval red in x in
+        change x with y
+  | |- equiv_coro' _ _ ?x =>
+    let y := eval red in x in
+        change x with y
+  | _ => idtac
+  end;
+  simpl;
+  lazymatch goal with
+    |- _ ?init _ =>
+    let u := open_constr:(inl env) in
+    unify init u
+  end;
+  let r := fresh in
+  repeat eexists; try econstructor;
+  [ intro r; derive_core open_constr:(fun x => inr x) (env,r)
+  | intros; dest_step'
+  ];
+  let ptr := next_ptr in
+  lazymatch goal with
+    |- equiv' _ _ (Return _ _ ?r) _ =>
+    eapply (Equiv'Return _ (ptr r));
+    simpl;
+    lazymatch goal with
+      |- _ ?a = _ =>
+      pattern_rhs a; apply eq_refl
+    end
+  | _ => idtac
+  end.
+
+Lemma ex_coroutine_derive :
+  { state & { step & forall k, { init | @equiv_coro' _ _ _ _ _ state step init (ex_coroutine k) }}}.
+  do 3 eexists.
+  derive_coro (tt,k).
 Defined.
 
+Definition ex_coroutine_step :=
+  projT1 (projT2 ex_coroutine_derive).
 
-Definition handshake pk sk :=
-  '(ourEphemeralPublic,ourEphemeralSecret) <- genKey;
-    print ourEphemeralPublic;
-      theirEphemeralPublic <- read;
-      theirHandshakeSealed <- read;
-      match open theirHandshakeSealed theirEphemeralPublic ourEphemeralSecret [1] with
-      | None => put 0; Pure _ tt
-      | Some theirHandshake =>
-        Let p := splitAt 32 theirHandshake in
-        Let theirPK := fst p in
-        Let theirHandshakeRest := snd p in
-        let hs := open theirHandshakeRest theirPK ourEphemeralSecret [2] in
-        let ourHandshake :=
-            pk ++ seal (ourEphemeralPublic ++ theirEphemeralPublic) theirEphemeralPublic sk [3]
-        in
-        print (seal ourHandshake theirPK ourEphemeralSecret [4]);
-          Pure _ tt
-      end.
+Definition ex_coroutine_equiv k :
+  equiv_coro' ex_coroutine_step _ (ex_coroutine k) :=
+  proj2_sig (projT2 (projT2 ex_coroutine_derive) k).
 
-Theorem handshake_derive :
-  {state & {step &
-            forall pk sk,
-              {init |
-               @equiv state _ step init (handshake pk sk) }}}.
+Definition ex_coroutine_equiv' k
+  : equiv_coro' ltac:(let x := eval simpl in (projT1 (projT2 ex_coroutine_derive)) in exact x) ltac:(let x := eval simpl in (proj1_sig (projT2 (projT2 ex_coroutine_derive) k)) in exact x) (ex_coroutine k) :=
+  ex_coroutine_equiv k.
+
+Hint Resolve ex_coroutine_equiv ex_coroutine_equiv' : equivc.
+Hint Resolve ex_coroutine_equiv : equivc'.
+
+Lemma GenForall2_nth_Some_list_equiv_coro :
+  forall (A B:Set) (IA : Inhabit A) (IB : Inhabit B) state
+         (step : step_type (const_yield A) (const_yield B) unit state)
+         x1 x2 n a1 a2,
+    GenForall2 (F := list)(fun (coro : coro_type step) (st : state) =>
+                  equiv_coro' step st coro) x1 x2 ->
+    nth_err _ x1 n = Some a1 ->
+    nth_err _ x2 n = Some a2 ->
+    equiv_coro' step a2 a1.
 Proof.
-  unfold handshake.
-  do 2 eexists.
   intros.
-  eexists ?[init].
-  let e := open_constr:(inl (tt,pk,sk)) in
-  unify ?init e.
-  derive' (tt,pk,sk).
-  derive' (tt,pk,sk,x,x1).
-  derive' (tt,pk,sk,x,x1,H).
+  eapply (GenForall2_nth_Some (F := list)(R := (fun (coro : coro_type step) (st : state) => equiv_coro' step st coro))); eauto.
+Qed.
+
+Hint Resolve GenForall2_nth_Some_list_equiv_coro : foldable.
+
+Ltac generalize_and_ind :=
+  lazymatch goal with
+    |- nat_rect_nondep _ _ ?k ?l = nat_rect_nondep _ _ _ ?l' =>
+    lazymatch type of l with
+    | context [@coro_type _ _ ?state ?step] =>
+        cut (GenForall2 (fun (coro : coro_type step) (st : state) => equiv_coro' step st coro) l l');
+      [ generalize l l'
+       |unfold GenForall2; eexists; split; [reflexivity|simpl; eauto with equivc]];
+      induction k; intros;
+      lazymatch goal with
+        |- nat_rect_nondep ?f ?f0 _ _ = nat_rect_nondep ?f' ?f0' _ _ =>
+        let tmp := fresh in
+        set (tmp := f);
+        let tmp' := fresh in
+        set (tmp' := f');
+        let tmp0 := fresh in
+        set (tmp0 := f0);
+        let tmp0' := fresh in
+        set (tmp0' := f0');
+        simpl nat_rect_nondep;
+        subst tmp; subst tmp'; subst tmp0; subst tmp0';
+        cbv beta
+      end
+    end
+  end.
+
+Ltac dest_yield :=
+  repeat match goal with
+         | e : yield_effect |- _ => destruct e
+         end.
+
+Ltac proc_step :=
+  lazymatch goal with
+    |- proc_coro ?c ?x ?f = step_state ?step ?st _ ?g =>
+    let H := fresh in
+    let H0 := fresh in
+    assert (equiv_coro' step st c) as (H,H0) by eauto with foldable;
+    let s := fresh "s" in
+    let e := fresh "e" in
+    let a := fresh "a" in
+    let p := fresh "p" in
+    let next := fresh "next" in
+    let op := fresh "op" in
+    let H1 := fresh in
+    let H2 := fresh in
+    inversion H0 as [s e a p next op H1 H2|];
+    subst;
+    unfold step_state at 1, seqE' at 1;
+    rewrite H2;
+    lazymatch goal with
+      |- context [match op ?x with _ => _ end] =>
+      specialize (H1 x);
+      destruct (op x);
+      inversion H1; subst;
+      unfold proc_coro at 1, seqE at 1;
+      lazymatch goal with
+        H_ : _ = c x |- _ =>
+        rewrite <- H_
+      end
+    end;
+    dest_yield
+  end.
+
+Ltac dest_opt :=
+  lazymatch goal with
+    |- match ?o with _ => _ end = option_branch _ _ ?o0 =>
+    destruct o eqn:?, o0 eqn:?;
+             unfold option_branch
+  end.
+
+Notation "'let_coro' x := c 'in' p" :=
+  (pipe (c : coro_type ltac:(let step := get_step c in exact step))
+        (fun x => p))
+    (at level 200, only parsing).
+
+Ltac mid_eq_core :=
+  generalize_and_ind
+  || dest_opt
+  || proc_step
+  || (repeat match goal with
+             | H : _ |- _ => apply H
+             end;
+      now eauto with foldable equivc)
+  || (exfalso; now eauto with foldable)
+  || reflexivity
+  || lazymatch goal with
+       |- Eff _ _ _ = Eff _ _ _ =>
+       f_equal;
+       let H := fresh in
+       extensionality H
+     end.
+
+Definition loop_ex (n i : nat) :=
+  let_coro c0 := ex_coroutine 0 in
+      nat_rect_nondep
+        (fun l =>
+           match nth_err _ l i : option (@coro_type nat nat _ _) with
+           | Some c =>
+             r <- resume c $ 1;
+               putN r;
+               Return _ _ (Some tt)
+           | None => Return _ _ None
+           end)
+        (fun m rec l =>
+           putN (0:args_effect putNat);
+             pipe (ex_coroutine m : @coro_type nat nat _ _)
+                  (fun cm =>
+                     rec (cm::l)))
+        n [c0].
+
+Ltac derive' env :=
+  lazymatch goal with
+    |- equiv _ ?init ?x =>
+    let u := open_constr:(inl env) in
+    unify init u;
+    repeat eexists;
+    [ dest_step'
+    | unfold option_branch;
+      derive_core open_constr:(fun a => inr a) env];
+    let ptr := next_ptr in
+    lazymatch goal with
+      |- equiv' ?step _ (Return _ _ ?r) _ =>
+      eapply (Equiv'Return _ (ptr r));
+      simpl;
+      lazymatch goal with
+        |- _ ?x = _ =>
+        pattern_rhs x;
+        apply eq_refl
+      | _ => apply eq_refl
+      end
+    end
+      (*
+      unshelve derive_core open_constr:(fun a => inr a) env;
+      intros; exact inhabitant*)
+  end.
+
+Definition simple_double_loop : t args_effect rets_effect _ :=
+  n <- getN;
+    nat_rect_nondep
+      (fun ls => Return _ _ (Some ls))
+      (fun n' rec ls =>
+         m <- getN;
+         nat_rect_nondep
+           (fun l => rec (l::ls))
+           (fun m' rec' l =>
+              k <- getN;
+                rec' (k::l))
+           m [])
+      n [].
+
+Definition simple_double_loop_derive :
+  { state & { step & { init | @equiv _ _ _ _ state step init simple_double_loop}}}.
+  do 3 eexists.
+  unfold simple_double_loop.
   derive' tt.
-  Grab Existential Variables.
-  all : exact unit || exact (fun _ => None ).
 Defined.
 
-Arguments existT {_ _}.
 
-Eval cbv [handshake_derive projT1 projT2 sum_merge prod_curry] in projT1 (projT2 handshake_derive).
+Eval cbv [projT1 projT2 simple_double_loop simple_double_loop_derive] in projT1 (projT2 simple_double_loop_derive).
+Arguments Return {_ _ _ _ } _.
+
+Definition list_ex :=
+  n <- getN;
+    list_rec_nondep
+      (fun a => Return (Some a))
+      (fun x l rec a =>
+         putN 0;
+         if Nat.even x then
+           rec (a + x)%nat
+         else
+           Return (Some a))
+      (seq 0 n) 0.
+
+Definition list_ex_derive :
+  { state & { step & { init | @equiv _ _ _ _ state step init list_ex}}}.
+Proof.
+  do 3 eexists.
+  unfold list_ex.
+  derive' tt.
+Defined.
+
+Definition simple_ex :=
+  n <- getN;
+    nat_rect_nondep
+      (fun accum => Return (Some accum))
+      (fun n' rec accum =>
+         putN n'; rec (n' + accum)%nat)
+      n 0.
 
 
-Definition handshake_step :=
-  Eval cbv [handshake_derive handshake projT2 projT1 sum_merge prod_curry] in projT1 (projT2 handshake_derive).
+Definition simple_ex_derive :
+  { state & { step & { init | @equiv _ _ _ _ state step init simple_ex}}}.
+  do 3 eexists.
+  unfold simple_ex.
+  derive' tt.
+Defined.
 
-Require Import Extraction.
+
+Eval cbv [projT1 projT2 simple_ex simple_ex_derive sum_merge prod_curry] in projT1 (projT2 simple_ex_derive).
+
+Definition dummy A (x : A) := True.
+
+Ltac list_unify def :=
+  lazymatch goal with
+    def := ?l |- ?c =>
+           let rec aux l :=
+               tryif is_evar l then
+                 let oc := open_constr:(c::_) in
+                 unify l oc
+               else
+                 lazymatch l with
+                 | _::?l' => aux l'
+                 end
+           in
+           aux l
+  end.
+
+Ltac state_to_nat s :=
+  lazymatch s with
+  | inr ?s' =>
+    let p := state_to_nat s' in
+    lazymatch p with
+      (?n,?v) =>
+      constr:((S n, v))
+    end
+  | inl ?v => constr:((O,v))
+  | ?v => constr:((O,v))
+  end.
+
+Ltac get_equalities l :=
+  match goal with
+  | _ : ?lhs = ?rhs |- _ =>
+    get_equalities constr:((lhs = rhs) :: l)
+  | _ => l
+  end.
+
+Ltac to_dot_core Heqp r :=
+  lazymatch type of Heqp with
+    _ = ?s0 =>
+    clear Heqp;
+    let p := state_to_nat s0 in
+    lazymatch p with
+      (?n0, ?v0) =>
+      let ty := type of v0 in
+      lazymatch goal with
+        |- dummy (inl (?s', ?op)) =>
+        let p := state_to_nat s' in
+        lazymatch p with
+          (?n, ?v) =>
+          lazymatch goal with
+          | EQR : r = ?r0 |- _ =>
+            clear EQR;
+            let eqs := get_equalities (@nil Prop) in
+            lazymatch goal with
+            | _ : dummy (n0, ty) |- _ =>
+              idtac
+            | _ => 
+              assert (dummy (n0, ty));
+              [ list_unify tt; exact I | ]
+            end;
+            change (dummy (n0, v0, r0, eqs, n, v, op));
+            repeat match goal with
+                     H : _ |- _ =>
+                     lazymatch goal with
+                       |- context[H] =>
+                       revert H
+                     end
+                   end
+          | _ =>
+            let eqs := get_equalities (@nil Prop) in
+            lazymatch goal with
+            | _ : dummy (n0, ty) |- _ =>
+              idtac
+            | _ => 
+              assert (dummy (n0, ty));
+              [ list_unify tt; exact I | ]
+            end;
+            change (dummy (n0, v0, r, eqs, n, v, op));
+            repeat match goal with
+                     H : _ |- _ =>
+                     lazymatch goal with
+                       |- context[H] =>
+                       revert H
+                     end
+                   end
+          end
+        end
+      | |- dummy (inr ?o) =>
+        lazymatch goal with
+        | _ : dummy (n0, ty) |- _ =>
+          idtac
+        | _ => 
+          assert (dummy (n0, ty));
+          [ list_unify tt; exact I | ]
+        end;
+        change (dummy (n0, v0, o));
+        repeat match goal with
+                 H : _ |- _ =>
+                 lazymatch goal with
+                   |- context[H] =>
+                   revert H
+                 end
+               end
+      end
+    end
+  end.
+
+Definition foo : list Prop.
+Proof.
+  evar (result : list Prop).
+  assert (forall s e r, dummy (projT1 (projT2 simple_ex_derive) s e r)).
+  intros.
+  destruct s eqn:?; simpl.
+  to_dot_core Heqp r.
+  list_unify result.
+  firstorder.
+  destruct s0; simpl.
+  destruct e.
+  destruct r eqn:?.
+  to_dot_core Heqp r.
+  list_unify result.
+  firstorder.
+  to_dot_core Heqp r.
+  list_unify result.
+  firstorder.
+  apply I.
+  apply I.
+  apply I.
+  apply I.
+  destruct s0; simpl.
+  destruct p; simpl.
+  destruct p; simpl.
+  destruct e.
+  apply I.
+  destruct n0.
+  to_dot_core Heqp r.
+  list_unify result.
+  firstorder.
+  to_dot_core Heqp r.
+  list_unify result.
+  firstorder.
+  apply I.
+  apply I.
+  apply I.
+  to_dot_core Heqp r.
+  list_unify result.
+  firstorder.
+  apply result.
+  Grab Existential Variables.
+  apply nil.
+Defined.
+Notation "<< x @ y @ .. @ z >>" :=
+  (dummy (pair .. (pair x y) .. z)) (at level 0).
+Eval cbv [foo] in foo.
+
+Ltac derive env :=
+  lazymatch goal with
+    |- equiv _ ?init ?x =>
+    let u := open_constr:(inl env) in
+    unify init u;
+    let H := fresh in
+    assert (x = ltac:(let x' := eval red in x in
+                          let x'' := coro_to_state x' in exact x''))
+      as H by
+         (change x with ltac:(let x0 := eval red in x in exact x0);
+            unfold pipe;
+            repeat mid_eq_core);
+    rewrite H;
+    clear H;
+    unfold step_state;
+    repeat eexists;
+    [ dest_step'
+    | unfold option_branch;
+      derive_core open_constr:(fun a => inr a) env ];
+    let ptr := next_ptr in
+    lazymatch goal with
+      |- equiv' ?step _ (Return ?r) _ =>
+      eapply (Equiv'Return _ (ptr r));
+      simpl;
+      lazymatch goal with
+        |- _ ?x = _ =>
+        pattern_rhs x;
+        apply eq_refl
+      | _ => apply eq_refl
+      end
+    end
+  end.
 
 
-Extraction Language Haskell.
+(*
+Lemma loop_ex_eq k n :
+  loop_ex k n =
+  ltac:(let x := (eval red in (loop_ex k n)) in
+        let x' := coro_to_state x in exact x').
+Proof.
+  unfold loop_ex.
+  unfold pipe.
+  repeat mid_eq_core.
+Qed.
+*)
 
-Extract Inductive unit => "()" [ "()" ].
-Extract Inductive list => "([])" ["[]" "(:)"].
-Extract Inductive bool => "Bool" ["True" "False"].
-Extract Inductive prod => "(,)"  [ "(,)" ].
-Extract Inductive sum => "Either" ["Left" "Right"].
-Extract Inductive option => "Maybe" ["Just" "Nothing"].
-Extract Inductive nat => Int ["0" "succ"] "(\fO fS n -> if n == 0 then fO () els e fS (n-1))".
+Definition loop_ex_derive n i :
+  { state & { step & { init | @equiv _ _ _ _ state step init (loop_ex n i) }}}.
+Proof.
+  do 3 eexists.
+  unshelve derive (tt,n,i); exact unit.
+Defined.
 
-Extract Inlined Constant splitAt => "Prelude.splitAt".
+Eval cbv [projT1 projT2 loop_ex_derive] in (fun n i => projT1 (projT2 (loop_ex_derive n i))).
 
-Extract Constant open =>
-  "\msg pk sk nonce -> boxOpen (fromJust $ decode $ BS.pack $ Prelude.map fromIntegral pk) (fromJust $ decode $ BS.pack $ Prelude.map fromIntegral sk) (fromJust $ decode $ BS.pack $ Prelude.map fromIntegral nonce) (BS.pack $ Prelude.map fromIntegral msg)".
-Extract Constant seal =>
-  "\msg pk sk nonce -> box (fromJust $ decode $ pack $ map fromIntegral pk) (fromJust $ decode $ pack $ map fromIntegral sk) (fromJust $ decode $ pack $ map fromIntegral nonce) (pack $ map fromIntegral msg)".
+Definition simple_ret : t args_effect rets_effect nat :=
+  n <- getN;
+    if Nat.even n then
+      Return 0
+    else
+      Return 1.
 
-Extraction "Handshake.hs" handshake_step.
+Definition simple_receive : t args_effect rets_effect (option unit) :=
+  x <<- simple_ret;
+    putN x;
+    Return (Some tt).
+
+Definition simple_derive :
+  { state & { step & { init | @equiv _ _ _ _ state step init simple_receive }}}.
+Proof.
+  do 3 eexists.
+  unfold simple_receive, simple_ret.
+  simpl.
+  derive' tt.
+Defined.
+
+(*
+Inductive tree A := Node : A -> tree A -> tree A -> tree A | Leaf.
+Instance tree_Inhabit A : Inhabit (tree A) :=
+  { inhabitant := Leaf _ }.
+
+Fixpoint insert A x a0 (t : tree (nat * A)) :=
+  match t with
+  | Node (y,a) l r =>
+    if Nat.leb x y then
+      Node (y,a) (insert x a0 l) r
+    else
+      Node (y,a) l (insert x a0 r)
+  | Leaf _ =>
+    Node (x,a0) (Leaf _) (Leaf _)
+  end.
+
+Fixpoint bsearch A key (t : tree (nat * A)) :=
+  match t with
+  | Node (x,a) l r =>
+    match Nat.compare key x with
+    | Eq => Some a
+    | Lt => bsearch key l
+    | Gt => bsearch key r
+    end
+  | Leaf _ => None
+  end.
+
+Fixpoint replace_map A key a0 (t : tree (nat * A)) :=
+  match t with
+  | Node (x,a) l r =>
+    match Nat.compare key x with
+    | Eq => Node (key,a0) l r
+    | Lt => Node (x,a) (replace_map key a0 l) r
+    | Gt => Node (x,a) l (replace_map key a0 r)
+    end
+  | Leaf _ => Leaf _
+  end.
+
+Fixpoint foldr_map A B (f : A -> B -> B)(init : B)(t : tree (nat * A)) :=
+  match t with
+  | Node (k,a) l r => foldr_map f (f a (foldr_map f init r)) l
+  | Leaf _ => init
+  end.
+
+Fixpoint zip_map A1 A2 (m1 : tree (nat * A1))(m2 : tree (nat * A2)) :=
+  match m1, m2 with
+  | Node (k1,a1) l1 r1, Node (k2,a2) l2 r2 =>
+    if Nat.eq_dec k1 k2 then
+      match zip_map l1 l2, zip_map r1 r2 with
+      | Some ml, Some mr =>
+        Some (Node (k1, (a1,a2)) ml mr)
+      | _,_ => None
+      end
+    else
+      None
+  | Leaf _, Leaf _ => Some (Leaf _)
+  | _, _ => None
+  end.
+
+Definition from_map_to_list A (t : tree (nat * A)) :=
+  foldr_map (fun a accum => a :: accum) [] t.
+
+Lemma fold_right_cons_app : forall A (l l0 : list A),
+    fold_right (fun a l' => a::l') l0 l = l ++ l0.
+Proof.
+  induction l; simpl; intros; congruence.
+Qed.
+
+Program Instance map_Foldable : Foldable (fun A => tree (nat * A)) :=
+  { foldr := foldr_map;
+    zip := zip_map;
+    to_list := from_map_to_list
+  }.
+Next Obligation.
+  intros.
+  unfold from_map_to_list.
+  revert B f b;
+  induction x; simpl in *; intros.
+  rewrite IHx2.
+  destruct a.
+  rewrite IHx1.
+  rewrite IHx1.
+  replace (f a
+       (fold_right f b
+                   (foldr_map (fun (a0 : A) (accum : list A) => a0 :: accum) [] x2)))
+  with (fold_right f b (a :: foldr_map (fun a0 accum => a0 :: accum) [] x2)) by auto.
+  rewrite <- fold_right_app.
+  f_equal.
+  setoid_rewrite IHx1 at 2.
+  setoid_rewrite IHx2 at 2.
+  replace ((a
+     :: fold_right (fun (a0 : A) (accum : list A) => a0 :: accum) []
+     (foldr_map (fun (a0 : A) (accum : list A) => a0 :: accum) [] x2)))
+  with (fold_right (fun (a0 : A) (accum : list A) => a0 :: accum) []
+                   (a ::foldr_map (fun (a0 : A) (accum : list A) => a0 :: accum) [] x2)) by auto.
+  rewrite <- fold_right_app.
+  rewrite fold_right_cons_app.
+  rewrite fold_right_cons_app.
+  do 2 rewrite app_nil_r.
+  auto.
+  auto.
+Qed.
+Next Obligation.
+  unfold from_map_to_list.
+  enough (forall l1 l2 l, zip_list l1 l2 = Some l ->
+                          Some
+    (foldr_map (fun (a : A1 * A2) (accum : list (A1 * A2)) => a :: accum) l x) =
+  zip_list (foldr_map (fun (a : A1) (accum : list A1) => a :: accum) l1 x1)
+    (foldr_map (fun (a : A2) (accum : list A2) => a :: accum) l2 x2)) by auto.
+  revert x x2 H.
+  induction x1; simpl in *; intros.
+  destruct a.
+  destruct x2; simpl in *; [|congruence].
+  destruct p.
+  destruct (Nat.eq_dec n n0); [|congruence].
+  subst.
+  destruct (zip_map x1_1 x2_1) eqn:?; simpl in *; [|congruence].
+  destruct (zip_map x1_2 x2_2) eqn:?; simpl in *; [|congruence].
+  inversion H. subst.
+  simpl.
+  eapply IHx1_1 in Heqo.
+  rewrite <- Heqo.
+  reflexivity.
+  simpl.
+  eapply IHx1_2 in Heqo0.
+  rewrite <- Heqo0.
+  simpl.
+  reflexivity.
+  auto.
+  destruct x2; [congruence|].
+  inversion H. subst.
+  auto.
+Qed.
+
+Lemma GenForall2_bsearch_Some_None : forall (A1 A2:Set) (R : A1 -> A2 -> Prop) m1 m2 k a,
+    GenForall2 R m1 m2 ->
+    bsearch k m1 = Some a ->
+    bsearch k m2 = None ->
+    False.
+Proof.
+  intros.
+  destruct H. destruct H.
+  clear H2.
+  revert x m2 H H1.
+  induction m1; intros; simpl in *.
+  destruct a0.
+  destruct m2.
+  destruct p.
+  simpl in H1.
+  destruct (k ?= n0) eqn:?.
+  congruence.
+  destruct (Nat.eq_dec n n0); [|congruence].
+  subst.
+  rewrite Heqc in H0.
+  destruct (zip_map m1_1 m2_1) eqn:?; [|congruence].
+  eauto.
+  destruct (Nat.eq_dec n n0); [|congruence].
+  subst.
+  rewrite Heqc in H0.
+  destruct (zip_map m1_1 m2_1) eqn:?; [|congruence].
+  destruct (zip_map m1_2 m2_2) eqn:?; [|congruence].
+  eauto.
+  congruence.
+  congruence.
+Qed.
+
+Lemma GenForall2_bsearch_None_Some : forall (A1 A2:Set) (R : A1 -> A2 -> Prop) m1 m2 k a,
+    GenForall2 R m1 m2 ->
+    bsearch k m1 = None ->
+    bsearch k m2 = Some a ->
+    False.
+Proof.
+  intros.
+  destruct H. destruct H.
+  clear H2.
+  revert x m2 H H1.
+  induction m1; intros; simpl in *.
+  destruct a0.
+  destruct m2; [|congruence].
+  destruct p.
+  destruct (Nat.eq_dec n n0); [|congruence].
+  subst.
+  simpl in H1.
+  destruct (k ?= n0) eqn:?.
+  congruence.
+  destruct (zip_map m1_1 m2_1) eqn:?; [|congruence].
+  destruct (zip_map m1_2 m2_2) eqn:?; [|congruence].
+  eauto.
+  destruct (zip_map m1_1 m2_1) eqn:?; [|congruence].
+  destruct (zip_map m1_2 m2_2) eqn:?; [|congruence].
+  eauto.
+  destruct m2.
+  congruence.
+  simpl in *.
+  congruence.
+Qed.
+
+Inductive Forall2_map A1 A2 (R : A1 -> A2 -> Prop) : tree (nat * A1) -> tree (nat * A2) -> Prop :=
+| FMLeaf : Forall2_map R (Leaf _) (Leaf _)
+| FMNode : forall k a1 a2 l1 l2 r1 r2,
+    R a1 a2 -> Forall2_map R l1 l2 -> Forall2_map R r1 r2 ->
+    Forall2_map R (Node (k, a1) l1 r1) (Node (k, a2) l2 r2).
+
+Lemma fold_right_and_Forall : forall (A:Set) (p : A -> Prop) l,
+    fold_right (fun a accum => p a /\ accum) True l ->
+    Forall p l.
+Proof.
+  induction l; intros; simpl in *.
+  auto.
+  econstructor; tauto.
+Qed.
+
+Lemma Forall_fold_right_and : forall (A:Set) (p : A -> Prop) p0 l,
+    p0 /\ Forall p l -> fold_right (fun a accum => p a /\ accum) p0 l.
+Proof.
+  induction l; simpl; intros.
+  tauto.
+  destruct H.
+  inversion H0. subst.
+  tauto.
+Qed.
+
+Lemma fold_map_app : forall A t (l : list A),
+    foldr_map (fun (a : A) accum => a :: accum) l t
+    = foldr_map (fun a accum => a :: accum) [] t ++ l.
+Proof.
+  induction t0; simpl; intros.
+  destruct a.
+  rewrite IHt0_2.
+  rewrite IHt0_1.
+  setoid_rewrite IHt0_1 at 2.
+  rewrite <- app_assoc.
+  simpl.
+  auto.
+  auto.
+Qed.
+
+Tactic Notation "eapply" "->" constr(lemma) "in" hyp(J) :=
+  bapply lemma ltac:(fun H => destruct H as [H _]; eapply H in J).
+
+Lemma Forall_appl : forall A l1 l2 (P : A -> Prop),
+    Forall P (l1 ++ l2) -> Forall P l1.
+Proof.
+  intros.
+  apply <- Forall_forall.
+  intros.
+  eapply -> Forall_forall in H; eauto.
+  apply in_or_app. auto.
+Qed.
+
+Lemma Forall_appr : forall A l1 l2 (P : A -> Prop),
+    Forall P (l1 ++ l2) -> Forall P l2.
+Proof.
+  intros.
+  apply <- Forall_forall.
+  intros.
+  eapply -> Forall_forall in H; eauto.
+  apply in_or_app. auto.
+Qed.
+
+Lemma GenForall2_Forall2_map : forall (A1 A2:Set) (R : A1 -> A2 -> Prop) m1 m2,
+    GenForall2 R m1 m2 <-> Forall2_map R m1 m2.
+Proof.
+  intros.
+  split.
+  intros.
+  destruct H.
+  destruct H.
+  replace (fun '(a1, a2) (p : Prop) => R a1 a2 /\ p) with
+  (fun a p => prod_curry R a /\ p) in H0.
+  all:swap 1 2.
+  unfold prod_curry.
+  extensionality a0.
+  extensionality p.
+  destruct a0.
+  auto.
+  apply fold_right_and_Forall in H0.
+  revert m2 x H H0.
+  induction m1; intros.
+  destruct m2; simpl in *.
+  destruct a.
+  destruct p.
+  destruct (Nat.eq_dec n n0); [|congruence].
+  subst.
+  destruct (zip_map m1_1 m2_1) eqn:?; [|congruence].
+  destruct (zip_map m1_2 m2_2) eqn:?; [|congruence].
+  inversion H.
+  subst.
+  econstructor.
+  unfold from_map_to_list in H0.
+  simpl in H0.
+  eapply -> Forall_forall in H0.
+  change (prod_curry R (a,a0)).
+  apply H0.
+  assert (In (a,a0) ((a, a0)
+        :: foldr_map
+        (fun (a1 : A1 * A2) (accum : list (A1 * A2)) => a1 :: accum) [] t1))
+    by intuition.
+  revert H1.
+  generalize ((a,a0) :: foldr_map (fun  (a1 : A1 * A2) (accum : list (A1 * A2)) => a1 :: accum) [] t1).
+  clear H H0 Heqo.
+  induction t0; simpl; intros.
+  destruct a1.
+  apply IHt0_1; simpl; auto.
+  auto.
+  eapply IHm1_1.
+  eauto.
+  unfold from_map_to_list in *.
+  simpl in H0.
+  rewrite fold_map_app in H0.
+  apply Forall_appl in H0.
+  auto.
+  eapply IHm1_2.
+  eauto.
+  unfold from_map_to_list in H0.
+  simpl in H0.
+  rewrite fold_map_app in H0.
+  apply Forall_appr in H0.
+  inversion H0. subst.
+  apply H4.
+  destruct a. congruence.
+  destruct m2.
+  simpl in H.
+  congruence.
+  econstructor.
+  simpl in *.
+  revert m2.
+  unfold GenForall2.
+  induction m1; simpl; intros.
+  inversion H. subst.
+  apply IHm1_1 in H5.
+  apply IHm1_2 in H6.
+  destruct H5.
+  destruct H0.
+  destruct H6.
+  destruct H2.
+  exists (Node (k,(a1,a2)) x x0).
+  split.
+  simpl.
+  destruct (Nat.eq_dec k k); [|congruence].
+  unfold zip in *.
+  simpl in *.
+  rewrite H0.
+  rewrite H2.
+  auto.
+  simpl.
+  unfold from_map_to_list.
+  simpl.
+  rewrite fold_map_app.
+  rewrite fold_right_app.
+  simpl.
+  unfold to_list in *.
+  simpl in *.
+  unfold from_map_to_list in *.
+  replace (fun '(a1,a2) p => R a1 a2 /\ p) with
+  (fun (a : A1 * A2) p => (let (a1,a2) := a in R a1 a2) /\ p) in *.
+  apply fold_right_and_Forall in H1.
+  apply Forall_fold_right_and.
+  repeat split; auto.
+  extensionality a.
+  destruct a.
+  auto.
+  exists (Leaf _).
+  inversion H.
+  split; simpl; auto.
+Qed.
+
+Lemma GenForall2_bsearch_Some : forall (A1 A2:Set) (R : A1 -> A2 -> Prop) m1 m2 k a1 a2,
+    GenForall2 R m1 m2 ->
+    bsearch k m1 = Some a1 ->
+    bsearch k m2 = Some a2 ->
+    R a1 a2.
+Proof.
+  intros.
+  apply GenForall2_Forall2_map in H.
+  revert m2 a1 a2 H H0 H1.
+  induction m1; simpl in *; intros.
+  inversion H. subst.
+  simpl in H1.
+  destruct (k ?= k0) eqn:?.
+  inversion H0. subst.
+  inversion H1. subst.
+  auto.
+  eauto.
+  eauto.
+  congruence.
+Qed.
+*)
+
+Lemma GenForall2_bsearch_Some_equiv_coro :
+  forall (A B : Set) (IA : Inhabit A) (IB : Inhabit B) (state : Set)
+         (step : step_type (const_yield A) (const_yield B) unit state)
+         x1 x2 n a1 a2,
+    GenForall2 (fun (coro : coro_type step) (st : state) => equiv_coro' step st coro) x1 x2 ->
+    bsearch n x1 = Some a1 ->
+    bsearch n x2 = Some a2 ->
+    equiv_coro' step a2 a1.
+Proof.
+  intros.
+  eapply (GenForall2_bsearch_Some (R := fun c s => equiv_coro' step s c)).
+  apply H.
+  eauto.
+  eauto.
+Qed.
+
+Hint Resolve GenForall2_bsearch_Some_equiv_coro : foldable.
+
+
+Definition coro_map_loop fuel :=
+  let_coro c := ex_coroutine 0 in
+        nat_rect_nondep
+          (fun _ => Return (Some tt))
+          (fun _ rec m' =>
+             key <- getStr;
+               match bsearch key m' : option (@coro_type nat nat _ _) with
+               | Some c =>
+                 n <- getN;
+                   r <- resume c $ n;
+                   putN r;
+                   rec (replace_map key c m')
+               | None => rec m'
+               end)
+          fuel (Node ("key",c) (Leaf _) (Leaf _)).
+
+Hint Constructors ex equiv'.
+Hint Unfold equiv_coro'.
+
+(*
+Lemma coro_map_loop_eq : forall fuel,
+    coro_map_loop fuel =
+    ltac:(let x := (eval red in (coro_map_loop fuel)) in
+          let x' := coro_to_state x in exact x').
+Proof.
+  intros.
+  unfold coro_map_loop, pipe.
+  repeat mid_eq_core.
+Qed.
+ *)
+
+Lemma coro_map_loop_derive : forall fuel,
+    { state & { step & { init | @equiv _ _ _  _ state step init (coro_map_loop fuel) }}}.
+Proof.
+  intros.
+  do 3 eexists.
+  unshelve derive (tt,fuel); exact inhabitant.
+Defined.
+
+
+Definition echo name s :
+  t (const_yield String.string) (const_yield String.string) unit :=
+  s' <- yield (String.append (String.append s " from ") name);
+    _ <- yield (String.append (String.append s' " from ") name);
+    Return tt.
+
+Lemma echo_derive :
+  { state & { step & forall name, { init | @equiv_coro' _ _ _ _ _ state step init (echo name) }}}.
+Proof.
+  do 3 eexists.
+  unshelve derive_coro (tt,name); exact inhabitant.
+Defined.
+
+Definition echo_step := projT1 (projT2 echo_derive).
+
+Definition echo_equiv n : equiv_coro' echo_step _ (echo n) :=
+  proj2_sig (projT2 (projT2 echo_derive) n).
+
+Definition echo_equiv' n
+  : equiv_coro' ltac:(let x := eval simpl in (projT1 (projT2 echo_derive)) in exact x) ltac:(let x := eval simpl in (proj1_sig (projT2 (projT2 echo_derive) n)) in exact x) (echo n) :=
+  echo_equiv n.
+
+Hint Resolve echo_equiv echo_equiv' : equivc equivc'.
+Hint Resolve echo_equiv : equivc'.
+
+Definition sendHello fuel :=
+  let_coro c0 := echo "c0" in
+  let_coro c1 := echo "c1" in
+  nat_rect_nondep
+    (fun _ => Return (Some tt))
+    (fun _ rec m =>
+       key <- getStr;
+         match bsearch key m : option (@coro_type String.string String.string _ _) with
+         | Some c =>
+           r <- resume c $ "hello";
+             putStr r;
+             rec (replace_map key c m)
+         | None => rec m
+         end)
+    fuel (Node ("key0",c0) (Node ("key1",c1) (Leaf _) (Leaf _)) (Leaf _)).
+
+(*
+Lemma sendHello_eq : forall fuel,
+    sendHello fuel =
+    ltac:(let x := (eval red in (sendHello fuel)) in
+          let x' := coro_to_state x in exact x').
+Proof.
+  intros.
+  unfold sendHello, pipe.
+  repeat mid_eq_core.
+Qed.
+ *)
+
+Lemma sendHello_derive fuel :
+  {state & {step & {init | @equiv _ _ _ _ state step init (sendHello fuel)}}}.
+Proof.
+  do 3 eexists.
+  unshelve derive (tt,fuel); exact inhabitant.
+Defined.
+
