src/Foldable.v
@@ -1,0 +1,688 @@
+Require Import List PeanoNat FunctionalExtensionality Inhabit.
+Require String Ascii.
+Import ListNotations.
+Import String.StringSyntax.
+Set Implicit Arguments.
+Open Scope type_scope.
+Open Scope string_scope.
+
+Fixpoint zip_list A1 A2 (l1 : list A1)(l2 : list A2) : option (list (A1 * A2)):=
+  match l1, l2 with
+  | [], [] => Some []
+  | a1::l1', a2::l2' =>
+    option_map (fun l => (a1,a2) :: l) (zip_list l1' l2')
+  | _, _ => None
+  end.
+
+Class Foldable (F : Set -> Set) :=
+  { foldr : forall (A B : Set), (A -> B -> B) -> B -> F A -> B;
+    zip : forall (A1 A2 : Set), F A1 -> F A2 -> option (F (A1 * A2));
+    to_list : forall A:Set, F A -> list A;
+    to_list_foldr : forall (A B:Set) (f : A -> B -> B) b x,
+        foldr f b x = fold_right f b (to_list x);
+    zip_to_list : forall (A1 A2 :Set)(x1 : F A1)(x2 : F A2) x,
+        zip x1 x2 = Some x -> Some (to_list x) = zip_list (to_list x1) (to_list x2)
+  }.
+
+Program Instance list_Foldable : Foldable list :=
+  { foldr := fun A B => @fold_right B A;
+    zip := zip_list;
+    to_list := fun _ x => x
+  }.
+
+Definition size A F `{F_Foldable : Foldable F} (x : F A) : (nat : Set) :=
+  foldr (fun _ accum => S accum) 0 x.
+
+Definition nth_err A F `{F_Foldable : Foldable F}(x : F A) :=
+  foldr (fun a p n =>
+           match n with
+           | O => Some a
+           | S n' => p n'
+           end)
+        (fun _ => None) x.
+
+Definition GenForall2 (A1 A2:Set) (F: Set -> Set) `{F_Foldable : Foldable F}
+           (R : A1 -> A2 -> Prop) (x1 : F A1) (x2 : F A2) :=
+  exists x, zip _ _ x1 x2 = Some x /\ fold_right (fun '(a1, a2) (p:Prop) => R a1 a2 /\ p) True (to_list _ x).
+
+Lemma GenForall2_cons : forall (A1 A2 :Set)(R : A1 -> A2 -> Prop) (x1 : list A1) (x2 : list A2) a1 a2,
+    R a1 a2 ->
+    GenForall2 R x1 x2 ->
+    GenForall2 R (a1::x1) (a2::x2).
+Proof.
+  unfold GenForall2. simpl.
+  intros.
+  destruct H0 as (x,(H1,H2)).
+  exists ((a1,a2) :: x).
+  split.
+  rewrite H1.
+  auto.
+  simpl.
+  auto.
+Qed.
+
+Lemma nth_err_nth_error : forall (A:Set) F (F_Foldable : Foldable F) (x : F A) n,
+    nth_err _ x n = nth_error (to_list _ x) n.
+Proof.
+  intros.
+  unfold nth_err.
+  rewrite to_list_foldr.
+  revert n.
+  induction (to_list A x); intros; simpl.
+  destruct n; auto.
+  destruct n; simpl; auto.
+Qed.
+
+Lemma size_length : forall (A:Set) F (F_Foldable : Foldable F) (x : F A),
+    size _ x = length (to_list _ x).
+Proof.
+  intros.
+  unfold size.
+  rewrite to_list_foldr.
+  induction (to_list _ x); simpl; auto.
+Qed.
+
+Lemma nth_err_Some : forall (A:Set) (F : Set -> Set) (F_Foldable : Foldable F) (x : F A) n a,
+    nth_err _ x n = Some a ->
+    n < size _ x.
+Proof.
+  intros.
+  unfold size, nth_err in *.
+  rewrite to_list_foldr in *.
+  revert n a H.
+  induction (to_list _ x); simpl; intros.
+  congruence.
+  destruct n.
+  auto with arith.
+  apply -> PeanoNat.Nat.succ_lt_mono.
+  eauto.
+Qed.
+
+Lemma nth_err_None : forall (A:Set) F (F_Foldable : Foldable F) (x : F A) n,
+    nth_err _ x n = None ->
+    ~ n < size _ x.
+Proof.
+  intros.
+  unfold size, nth_err in *.
+  rewrite to_list_foldr in *.
+  revert n H.
+  induction (to_list _ x); simpl; intros.
+  auto with arith.
+  destruct n.
+  congruence.
+  apply IHl in H.
+  auto with arith.
+Qed.
+
+Lemma GenForall2_Forall2 : forall (A1 A2:Set) F (F_Foldable : Foldable F) R (x1 : F A1) (x2 : F A2),
+    GenForall2 R x1 x2 -> Forall2 R (to_list _ x1) (to_list _ x2).
+Proof.
+  intros.
+  unfold GenForall2 in H.
+  destruct H as (x,(H0,H1)).
+  apply zip_to_list in H0.
+  generalize dependent (to_list _ x).
+  generalize (to_list A2 x2).
+  induction (to_list _ x1); intros.
+  destruct l.
+  auto.
+  simpl in H0.
+  congruence.
+  destruct l0.
+  simpl in H0.
+  congruence.
+  simpl in *.
+  destruct (zip_list l l0) eqn:?.
+  simpl in *.
+  symmetry in Heqo.
+  inversion H0. subst.
+  simpl in H1.
+  econstructor.
+  tauto.
+  apply IHl in Heqo.
+  auto.
+  tauto.
+  simpl in H0.
+  congruence.
+Qed.
+
+Lemma GenForall2_size : forall (A1 A2 : Set) (F : Set -> Set) (F_Foldable : Foldable F) R (x1 : F A1) (x2 : F A2),
+    GenForall2 R x1 x2 ->
+    size _ x1 = size _ x2.
+Proof.
+  intros.
+  destruct H.
+  destruct H.
+  apply zip_to_list in H.
+  unfold size.
+  repeat rewrite to_list_foldr in *.
+  generalize dependent (to_list _ x2).
+  generalize dependent (to_list _ x).
+  induction (to_list _ x1); simpl in *; intros.
+  destruct l0; simpl in *; congruence.
+  destruct l1; simpl in *.
+  congruence.
+  f_equal.
+  destruct (zip_list l l1) eqn:?; simpl in *.
+  apply (IHl l2).
+  inversion H. subst.
+  simpl in H0.
+  tauto.
+  inversion H. subst.
+  auto.
+  congruence.
+Qed.
+
+Lemma GenForall2_nth_Some_None : forall (A1 A2 : Set) R (x1 : list A1) (x2 : list A2) n a1,
+    GenForall2 (F := list) R x1 x2 ->
+    nth_err _ x1 n = Some a1 ->
+    nth_err _ x2 n = None ->
+    False.
+Proof.
+  intros.
+  apply nth_err_None in H1.
+  apply nth_err_Some in H0.
+  apply GenForall2_size in H.
+  rewrite H in H0.
+  auto.
+Qed.
+
+Lemma GenForall2_nth_None_Some : forall (A1 A2 : Set) R (x1 : list A1) (x2 : list A2) n a2,
+    GenForall2 (F := list) R x1 x2 ->
+    nth_err _ x1 n = None ->
+    nth_err _ x2 n = Some a2 ->
+    False.
+Proof.
+  intros.
+  apply nth_err_Some in H1.
+  apply nth_err_None in H0.
+  apply GenForall2_size in H.
+  rewrite H in H0.
+  auto.
+Qed.
+
+Lemma GenForall2_nth_Some : forall (A1 A2 : Set) (F : Set -> Set) (F_Foldable : Foldable F) R (x1 : F A1) (x2 : F A2) n a1 a2,
+    GenForall2 R x1 x2 ->
+    nth_err _ x1 n = Some a1 ->
+    nth_err _ x2 n = Some a2 ->
+    R a1 a2.
+Proof.
+  intros.
+  unfold nth_err in *.
+  unfold GenForall2 in H.
+  destruct H.
+  destruct H.
+  unfold size in H.
+  rewrite to_list_foldr in H0.
+  rewrite to_list_foldr in H1.
+  apply zip_to_list in H.
+  generalize dependent (to_list _ x2).
+  generalize dependent (to_list _ x).
+  revert n a1 a2 H0.
+  induction (to_list _ x1); simpl in *; intros.
+  destruct l0.
+  inversion H. subst.
+  simpl in H1.
+  congruence.
+  congruence.
+  destruct l1; [congruence|].
+  destruct (zip_list l l1) eqn:?; simpl in *; [|congruence].
+  inversion H. subst.
+  simpl in H2.
+  destruct n.
+  inversion H0. subst.
+  inversion H1. subst.
+  tauto.
+  destruct H2.
+  eapply IHl.
+  eauto.
+  eauto.
+  symmetry. eauto.
+  auto.
+Qed.
+
+Hint Resolve GenForall2_size nth_err_None nth_err_Some GenForall2_cons GenForall2_nth_None_Some GenForall2_nth_Some_None : foldable.
+
+
+Inductive Map A := Node : String.string * A -> Map A -> Map A -> Map A | Leaf.
+
+Definition compareAscii (x y : Ascii.ascii) :=
+  Nat.compare (Ascii.nat_of_ascii x) (Ascii.nat_of_ascii y).
+
+Fixpoint compareString (x y : String.string) :=
+  match x, y with
+  | String.EmptyString, String.EmptyString => Eq
+  | String.EmptyString, _ => Lt
+  | _, String.EmptyString => Gt
+  | String.String c x', String.String d y' =>
+    match compareAscii c d with
+    | Eq => compareString x' y'
+    | Lt => Lt
+    | Gt => Gt
+    end
+  end.
+
+Definition lebString (x y : String.string) :=
+  match compareString x y with
+  | Gt => false
+  | _ => true
+  end.
+
+Fixpoint insert A x a0 (t : Map A) :=
+  match t with
+  | Node (y,a) l r =>
+    if lebString x y then
+      Node (y,a) (insert x a0 l) r
+    else
+      Node (y,a) l (insert x a0 r)
+  | Leaf _ =>
+    Node (x,a0) (Leaf _) (Leaf _)
+  end.
+
+Fixpoint bsearch A key (t : Map A) :=
+  match t with
+  | Node (x,a) l r =>
+    match compareString key x with
+    | Eq => Some a
+    | Lt => bsearch key l
+    | Gt => bsearch key r
+    end
+  | Leaf _ => None
+  end.
+
+Fixpoint replace_map A key a0 (t : Map A) :=
+  match t with
+  | Node (x,a) l r =>
+    match compareString key x with
+    | Eq => Node (key,a0) l r
+    | Lt => Node (x,a) (replace_map key a0 l) r
+    | Gt => Node (x,a) l (replace_map key a0 r)
+    end
+  | Leaf _ => Leaf _
+  end.
+
+Fixpoint foldr_map (A B:Set) (f : A -> B -> B)(init : B)(t : Map A) :=
+  match t with
+  | Node (k,a) l r => foldr_map f (f a (foldr_map f init r)) l
+  | Leaf _ => init
+  end.
+
+Fixpoint zip_map A1 A2 (m1 : Map A1)(m2 : Map A2) :=
+  match m1, m2 with
+  | Node (k1,a1) l1 r1, Node (k2,a2) l2 r2 =>
+    if String.string_dec k1 k2 then
+      match zip_map l1 l2, zip_map r1 r2 with
+      | Some ml, Some mr =>
+        Some (Node (k1, (a1,a2)) ml mr)
+      | _,_ => None
+      end
+    else
+      None
+  | Leaf _, Leaf _ => Some (Leaf _)
+  | _, _ => None
+  end.
+
+Definition from_map_to_list (A:Set) (t : Map A) :=
+  foldr_map (fun a accum => a :: accum) [] t.
+
+Lemma fold_right_cons_app : forall A (l l0 : list A),
+    fold_right (fun a l' => a::l') l0 l = l ++ l0.
+Proof.
+  induction l; simpl; intros; congruence.
+Qed.
+
+Lemma to_list_foldr_map : forall (A B : Set) (f : A -> B -> B) (b : B) (x : Map A),
+    foldr_map f b x = fold_right f b (from_map_to_list x).
+Proof.
+  intros.
+  unfold from_map_to_list.
+  revert B f b;
+  induction x; simpl in *; intros.
+  rewrite IHx2.
+  destruct p.
+  rewrite IHx1.
+  rewrite IHx1.
+  replace (f a
+       (fold_right f b
+                   (foldr_map (fun (a0 : A) (accum : list A) => a0 :: accum) [] x2)))
+  with (fold_right f b (a :: foldr_map (fun a0 accum => a0 :: accum) [] x2)) by auto.
+  rewrite <- fold_right_app.
+  f_equal.
+  setoid_rewrite IHx1 at 2.
+  setoid_rewrite IHx2 at 2.
+  replace ((a
+     :: fold_right (fun (a0 : A) (accum : list A) => a0 :: accum) []
+     (foldr_map (fun (a0 : A) (accum : list A) => a0 :: accum) [] x2)))
+  with (fold_right (fun (a0 : A) (accum : list A) => a0 :: accum) []
+                   (a ::foldr_map (fun (a0 : A) (accum : list A) => a0 :: accum) [] x2)) by auto.
+  rewrite <- fold_right_app.
+  rewrite fold_right_cons_app.
+  rewrite fold_right_cons_app.
+  do 2 rewrite app_nil_r.
+  auto.
+  auto.
+Qed.
+
+Lemma zip_to_list_map : forall (A1 A2 : Set) (x1 : Map A1) (x2 : Map A2) (x : Map (A1 * A2)),
+                  zip_map x1 x2 = Some x ->
+                  Some (from_map_to_list x) =
+                  zip_list (from_map_to_list x1) (from_map_to_list x2).
+Proof.
+  unfold from_map_to_list.
+  intros.
+  enough (forall l1 l2 l, zip_list l1 l2 = Some l ->
+                          Some
+    (foldr_map (fun (a : A1 * A2) (accum : list (A1 * A2)) => a :: accum) l x) =
+  zip_list (foldr_map (fun (a : A1) (accum : list A1) => a :: accum) l1 x1)
+    (foldr_map (fun (a : A2) (accum : list A2) => a :: accum) l2 x2)) by auto.
+  revert x x2 H.
+  induction x1; simpl in *; intros.
+  destruct p.
+  destruct x2; simpl in *; [|congruence].
+  destruct p.
+  destruct (String.string_dec s s0); [|congruence].
+  subst.
+  destruct (zip_map x1_1 x2_1) eqn:?; simpl in *; [|congruence].
+  destruct (zip_map x1_2 x2_2) eqn:?; simpl in *; [|congruence].
+  inversion H. subst.
+  simpl.
+  eapply IHx1_1 in Heqo.
+  rewrite <- Heqo.
+  reflexivity.
+  simpl.
+  eapply IHx1_2 in Heqo0.
+  rewrite <- Heqo0.
+  simpl.
+  reflexivity.
+  auto.
+  destruct x2; [congruence|].
+  inversion H. subst.
+  auto.
+Qed.
+
+Instance map_Foldable : Foldable Map :=
+  { foldr := foldr_map;
+    zip := zip_map;
+    to_list := from_map_to_list;
+    to_list_foldr := to_list_foldr_map;
+    zip_to_list := zip_to_list_map
+  }.
+
+
+Lemma GenForall2_bsearch_Some_None : forall (A1 A2:Set) (R : A1 -> A2 -> Prop) m1 m2 k a,
+    GenForall2 R m1 m2 ->
+    bsearch k m1 = Some a ->
+    bsearch k m2 = None ->
+    False.
+Proof.
+  intros.
+  destruct H. destruct H.
+  clear H2.
+  revert x m2 H H1.
+  induction m1; intros; simpl in *.
+  destruct p.
+  destruct m2.
+  destruct p.
+  simpl in H1.
+  destruct (compareString k s0) eqn:?.
+  congruence.
+  destruct (String.string_dec s s0); [|congruence].
+  subst.
+  rewrite Heqc in H0.
+  destruct (zip_map m1_1 m2_1) eqn:?; [|congruence].
+  eauto.
+  destruct (String.string_dec s s0); [|congruence].
+  subst.
+  rewrite Heqc in H0.
+  destruct (zip_map m1_1 m2_1) eqn:?; [|congruence].
+  destruct (zip_map m1_2 m2_2) eqn:?; [|congruence].
+  eauto.
+  congruence.
+  congruence.
+Qed.
+
+Lemma GenForall2_bsearch_None_Some : forall (A1 A2:Set) (R : A1 -> A2 -> Prop) m1 m2 k a,
+    GenForall2 R m1 m2 ->
+    bsearch k m1 = None ->
+    bsearch k m2 = Some a ->
+    False.
+Proof.
+  intros.
+  destruct H. destruct H.
+  clear H2.
+  revert x m2 H H1.
+  induction m1; intros; simpl in *.
+  destruct p.
+  destruct m2; [|congruence].
+  destruct p.
+  destruct (String.string_dec s s0); [|congruence].
+  subst.
+  simpl in H1.
+  destruct (compareString k s0) eqn:?.
+  congruence.
+  destruct (zip_map m1_1 m2_1) eqn:?; [|congruence].
+  destruct (zip_map m1_2 m2_2) eqn:?; [|congruence].
+  eauto.
+  destruct (zip_map m1_1 m2_1) eqn:?; [|congruence].
+  destruct (zip_map m1_2 m2_2) eqn:?; [|congruence].
+  eauto.
+  destruct m2.
+  congruence.
+  simpl in *.
+  congruence.
+Qed.
+
+Inductive Forall2_map (A1 A2:Set) (R : A1 -> A2 -> Prop) : Map A1 -> Map A2 -> Prop :=
+| FMLeaf : Forall2_map R (Leaf _) (Leaf _)
+| FMNode : forall k a1 a2 l1 l2 r1 r2,
+    R a1 a2 -> Forall2_map R l1 l2 -> Forall2_map R r1 r2 ->
+    Forall2_map R (Node (k, a1) l1 r1) (Node (k, a2) l2 r2).
+
+Lemma fold_right_and_Forall : forall (A:Set) (p : A -> Prop) l,
+    fold_right (fun a accum => p a /\ accum) True l ->
+    Forall p l.
+Proof.
+  induction l; intros; simpl in *.
+  auto.
+  econstructor; tauto.
+Qed.
+
+Lemma Forall_fold_right_and : forall (A:Set) (p : A -> Prop) p0 l,
+    p0 /\ Forall p l -> fold_right (fun a accum => p a /\ accum) p0 l.
+Proof.
+  induction l; simpl; intros.
+  tauto.
+  destruct H.
+  inversion H0. subst.
+  tauto.
+Qed.
+
+Lemma fold_map_app : forall (A:Set) (t:Map A) (l : list A),
+    foldr_map (fun (a : A) accum => a :: accum) l t
+    = foldr_map (fun a accum => a :: accum) [] t ++ l.
+Proof.
+  induction t; simpl; intros.
+  destruct p.
+  rewrite IHt2.
+  rewrite IHt1.
+  setoid_rewrite IHt1 at 2.
+  rewrite <- app_assoc.
+  simpl.
+  auto.
+  auto.
+Qed.
+
+Tactic Notation "eapply" "->" constr(lemma) "in" hyp(J) :=
+  bapply lemma ltac:(fun H => destruct H as [H _]; eapply H in J).
+
+Lemma Forall_appl : forall A l1 l2 (P : A -> Prop),
+    Forall P (l1 ++ l2) -> Forall P l1.
+Proof.
+  intros.
+  apply <- Forall_forall.
+  intros.
+  eapply -> Forall_forall in H; eauto.
+  apply in_or_app. auto.
+Qed.
+
+Lemma Forall_appr : forall A l1 l2 (P : A -> Prop),
+    Forall P (l1 ++ l2) -> Forall P l2.
+Proof.
+  intros.
+  apply <- Forall_forall.
+  intros.
+  eapply -> Forall_forall in H; eauto.
+  apply in_or_app. auto.
+Qed.
+
+Lemma GenForall2_Forall2_map : forall (A1 A2:Set) (R : A1 -> A2 -> Prop) m1 m2,
+    GenForall2 R m1 m2 <-> Forall2_map R m1 m2.
+Proof.
+  intros.
+  split.
+  intros.
+  destruct H.
+  destruct H.
+  replace (fun '(a1, a2) (p : Prop) => R a1 a2 /\ p) with
+  (fun a p => prod_curry R a /\ p) in H0.
+  all:swap 1 2.
+  unfold prod_curry.
+  extensionality a0.
+  extensionality p.
+  destruct a0.
+  auto.
+  apply fold_right_and_Forall in H0.
+  revert m2 x H H0.
+  induction m1; intros.
+  destruct m2; simpl in *.
+  destruct p.
+  destruct p0.
+  destruct (String.string_dec s s0); [|congruence].
+  subst.
+  destruct (zip_map m1_1 m2_1) eqn:?; [|congruence].
+  destruct (zip_map m1_2 m2_2) eqn:?; [|congruence].
+  inversion H.
+  subst.
+  econstructor.
+  unfold from_map_to_list in H0.
+  simpl in H0.
+  eapply -> Forall_forall in H0.
+  change (prod_curry R (a,a0)).
+  apply H0.
+  assert (In (a,a0) ((a, a0)
+        :: foldr_map
+        (fun (a1 : A1 * A2) (accum : list (A1 * A2)) => a1 :: accum) [] m0))
+    by intuition.
+  revert H1.
+  generalize ((a,a0) :: foldr_map (fun  (a1 : A1 * A2) (accum : list (A1 * A2)) => a1 :: accum) [] m0).
+  clear H H0 Heqo.
+  induction m; simpl; intros.
+  destruct p.
+  apply IHm1; simpl; auto.
+  auto.
+  eapply IHm1_1.
+  eauto.
+  unfold from_map_to_list in *.
+  simpl in H0.
+  rewrite fold_map_app in H0.
+  apply Forall_appl in H0.
+  auto.
+  eapply IHm1_2.
+  eauto.
+  unfold from_map_to_list in H0.
+  simpl in H0.
+  rewrite fold_map_app in H0.
+  apply Forall_appr in H0.
+  inversion H0. subst.
+  apply H4.
+  destruct p. congruence.
+  destruct m2.
+  simpl in H.
+  congruence.
+  econstructor.
+  simpl in *.
+  revert m2.
+  unfold GenForall2.
+  induction m1; simpl; intros.
+  inversion H. subst.
+  apply IHm1_1 in H5.
+  apply IHm1_2 in H6.
+  destruct H5.
+  destruct H0.
+  destruct H6.
+  destruct H2.
+  exists (Node (k,(a1,a2)) x x0).
+  split.
+  simpl.
+  destruct (String.string_dec k k); [|congruence].
+  unfold zip in *.
+  simpl in *.
+  rewrite H0.
+  rewrite H2.
+  auto.
+  simpl.
+  unfold from_map_to_list.
+  simpl.
+  rewrite fold_map_app.
+  rewrite fold_right_app.
+  simpl.
+  unfold to_list in *.
+  simpl in *.
+  unfold from_map_to_list in *.
+  replace (fun '(a1,a2) p => R a1 a2 /\ p) with
+  (fun (a : A1 * A2) p => (let (a1,a2) := a in R a1 a2) /\ p) in *.
+  apply fold_right_and_Forall in H1.
+  apply Forall_fold_right_and.
+  repeat split; auto.
+  extensionality a.
+  destruct a.
+  auto.
+  exists (Leaf _).
+  inversion H.
+  split; simpl; auto.
+Qed.
+
+Lemma GenForall2_bsearch_Some : forall (A1 A2:Set) (R : A1 -> A2 -> Prop) m1 m2 k a1 a2,
+    GenForall2 R m1 m2 ->
+    bsearch k m1 = Some a1 ->
+    bsearch k m2 = Some a2 ->
+    R a1 a2.
+Proof.
+  intros.
+  apply GenForall2_Forall2_map in H.
+  revert m2 a1 a2 H H0 H1.
+  induction m1; simpl in *; intros.
+  inversion H. subst.
+  simpl in H1.
+  destruct (compareString k k0) eqn:?.
+  inversion H0. subst.
+  inversion H1. subst.
+  auto.
+  eauto.
+  eauto.
+  congruence.
+Qed.
+
+Lemma GenForall2_replace_map : forall (A B : Set)(R : A -> B -> Prop)(m1 : Map A) m2 a b n,
+    GenForall2 R m1 m2 ->
+    R a b ->
+    GenForall2 R (replace_map n a m1) (replace_map n b m2).
+Proof.
+  intros.
+  apply GenForall2_Forall2_map.
+  apply GenForall2_Forall2_map in H.
+  revert m2 a b n H H0.
+  induction m1; intros.
+  simpl.
+  destruct p.
+  inversion H. subst.
+  simpl.
+  destruct (compareString n s) eqn:?; constructor; auto.
+  inversion H. subst.
+  simpl.
+  constructor.
+Qed.
+
+Instance Map_inhabitant A : Inhabit (Map A) := { inhabitant := Leaf _ }.
+
+Hint Resolve GenForall2_bsearch_Some_None GenForall2_bsearch_None_Some GenForall2_replace_map : foldable.
