src/Inhabit.v
@@ -1,0 +1,31 @@
+Require String.
+
+Class Inhabit A := { inhabitant : A }.
+
+Definition dummy Idx A `{IA : Inhabit A} (i : Idx) : A := inhabitant.
+
+Instance nat_inhabit : Inhabit nat := { inhabitant := 0 }.
+
+Instance list_inhabit T : Inhabit (list T) := { inhabitant := @nil T }.
+
+Instance unit_inhabitant : Inhabit unit := {inhabitant := tt }.
+
+Instance prod_inhabitant A B `{IA : Inhabit A} `{IB : Inhabit B} : Inhabit (A * B) :=
+  { inhabitant := (inhabitant, inhabitant) }.
+
+Instance string_inhabitant : Inhabit String.string :=
+  { inhabitant := String.EmptyString }.
+
+Instance sum_inhabitant A B `{IA : Inhabit A} : Inhabit (A + B) :=
+  { inhabitant := inl inhabitant }.
+
+Instance arrow_inhabitant A B `{IB : Inhabit B} : Inhabit (A -> B) :=
+  { inhabitant := fun _:A => inhabitant }.
+
+Instance option_inhabitant A : Inhabit (option A) :=
+  { inhabitant := None }.
+Instance Set_inhabitant : Inhabit Set :=
+  { inhabitant := unit }.
+
+Instance Type_inhabitant : Inhabit Type :=
+  { inhabitant := unit }.
